fix

src/FOL/arithmetic.lean
@@ -84,14 +84,14 @@ local infix ` ≺ `:50 := additional.lt
 local infix ` ⍭ `:50 := additional.dvd
 
 inductive robinson : Theory LA
-| q1 : robinson ∀₁ x, 0 ≄ Succ x
-| q2 : robinson ∀₁ x, ∀₁ y, ((Succ x ≃ Succ y) ⟶ (x ≃ y))
-| q3 : robinson ∀₁ x, ((x ≃ 0) ⊔ ∃₁ y, x ≃ Succ y)
-| q4 : robinson ∀₁ x, x + 0 ≃ x
-| q5 : robinson ∀₁ x y, x + Succ y ≃ Succ (x + y)
-| q6 : robinson ∀₁ x, x * 0 ≃ 0
-| q7 : robinson ∀₁ x y, x * Succ y ≃ x * y + x
-| q8 : robinson ∀₁ x y, ((x ≼ y) ⟷ ∃₁ z, z + x ≃ y)
+| q1 : robinson ∀₁ x, 0 ≠' Succ x
+| q2 : robinson ∀₁ x, ∀₁ y, ((Succ x =' Succ y) ⟶ (x =' y))
+| q3 : robinson ∀₁ x, ((x =' 0) ⊔ ∃₁ y, x =' Succ y)
+| q4 : robinson ∀₁ x, x + 0 =' x
+| q5 : robinson ∀₁ x y, x + Succ y =' Succ (x + y)
+| q6 : robinson ∀₁ x, x * 0 =' 0
+| q7 : robinson ∀₁ x y, x * Succ y =' x * y + x
+| q8 : robinson ∀₁ x y, ((x ≼ y) ⟷ ∃₁ z, z + x =' y)
 
 notation `𝐐` := robinson
 
@@ -102,9 +102,9 @@ namespace additional
 instance addditional_predicate : additional.predicate := ⟨λ n, pempty.is_empty⟩
 
 @[simp] def df_pr : Π {n} (r : additional.pr n), formula LA
-| 2 additional_pr.lt := ((#0 : term LA) ≼ #1) ⊓ ((#0 : term LA) ≄ #1)
-| 2 additional_pr.dvd := ∃. (#0 * #1 ≃ #2)
-| 1 additional_pr.prime := ∃. (#0 + 1 ≃ #1) ⊓ ∀. (∃. (#0 * #2 ≃ #1) ⟶ (#0 ≃ 1) ⊔ (#0 ≃ #1))
+| 2 additional_pr.lt := ((#0 : term LA) ≼ #1) ⊓ ((#0 : term LA) ≠' #1)
+| 2 additional_pr.dvd := ∃. (#0 * #1 =' #2)
+| 1 additional_pr.prime := ∃. (#0 + 1 =' #1) ⊓ ∀. (∃. (#0 * #2 =' #1) ⟶ (#0 =' 1) ⊔ (#0 =' #1))
 
 @[reducible] def defs : LA.definitions additional :=
 { df_fn := λ n f, by exfalso; exact is_empty.false f,
@@ -114,10 +114,10 @@ instance addditional_predicate : additional.predicate := ⟨λ n, pempty.is_empt
 
 variables [LA'.language_translation_coe L] (T : Theory L) [lextend defs.thy T] {i : ℕ}
 
-@[simp] lemma thy.lt (x y) : T ⊢ (x ≺ y) ⟷ (x ≼ y) ⊓ (x ≄ y) :=
+@[simp] lemma thy.lt (x y) : T ⊢ (x ≺ y) ⟷ (x ≼ y) ⊓ (x ≠' y) :=
 by simpa[fal_fn] using defs.pr' T additional_pr.lt ‹x, y›
 
-@[simp] lemma thy.dvd (x y) : T ⊢ (x ⍭ y) ⟷ ∃. (#0 * x^1 ≃ y^1) :=
+@[simp] lemma thy.dvd (x y) : T ⊢ (x ⍭ y) ⟷ ∃. (#0 * x^1 =' y^1) :=
 by simpa[fal_fn, ex_fn] using defs.pr' T additional_pr.dvd ‹x, y›
 
 variables {T}
@@ -130,7 +130,7 @@ infix ` ≺' `:50 := Herbrand.lt
 @[simp] lemma Lindenbaum.lt_def (v) :
   Lindenbaum.predicate_of ((coe : LA'.pr 2 → L.pr 2) (sum.inr additional_pr.lt)) v = (v 0 ≺' v 1 : Lindenbaum T i) := rfl
 
-lemma Lindenbaum.lt_eq (h₁ h₂ : Herbrand T i) : (h₁ ≺' h₂) = (h₁ ≼ h₂) ⊓ (h₁ ≃ h₂)ᶜ :=
+lemma Lindenbaum.lt_eq (h₁ h₂ : Herbrand T i) : (h₁ ≺' h₂) = (h₁ ≼ h₂) ⊓ (h₁ =' h₂)ᶜ :=
 by induction h₁ using fol.Herbrand.ind_on with t;
    induction h₂ using fol.Herbrand.ind_on with u;
    simpa[lt] using Lindenbaum.eq_of_provable_equiv.mp (thy.lt _ t u)
@@ -143,7 +143,7 @@ infix ` ⍭' `:50 := Herbrand.dvd
 @[simp] lemma Lindenbaum.dvd_def (v) :
   Lindenbaum.predicate_of ((coe : LA'.pr 2 → L.pr 2) (sum.inr additional_pr.dvd)) v = (v 0 ⍭' v 1 : Lindenbaum T i) := rfl
 
-lemma Lindenbaum.dvd_eq (h₁ h₂ : Herbrand T i) : (h₁ ⍭' h₂) = ∃' (♯0 * h₁.pow ≃ h₂.pow : Lindenbaum T (i + 1)) :=
+lemma Lindenbaum.dvd_eq (h₁ h₂ : Herbrand T i) : (h₁ ⍭' h₂) = ∃' (♯0 * h₁.pow =' h₂.pow : Lindenbaum T (i + 1)) :=
 by induction h₁ using fol.Herbrand.ind_on with t;
    induction h₂ using fol.Herbrand.ind_on with u;
    simpa[dvd] using Lindenbaum.eq_of_provable_equiv.mp (thy.dvd _ t u)
@@ -214,26 +214,26 @@ namespace robinson
 open Herbrand Lindenbaum provable
 variables {L} [LA.language_translation_coe L] (Q : Theory L) [lextend 𝐐 Q] (i : ℕ)
 
-@[simp] lemma zero_ne_succ (t : term L) : Q ⊢ 0 ≄ Succ t :=
-by { have : Q ⊢ ∀₁ x, 0 ≄ Succ x, by simpa[fal_fn] using provable.lextend (by_axiom robinson.q1) Q,
+@[simp] lemma zero_ne_succ (t : term L) : Q ⊢ 0 ≠' Succ t :=
+by { have : Q ⊢ ∀₁ x, 0 ≠' Succ x, by simpa[fal_fn] using provable.lextend (by_axiom robinson.q1) Q,
      simpa using this ⊚ t }
 
-@[simp] lemma Lindembaum.zero_ne_succ (h : Herbrand Q i) : 0 ≃ Succ h = (⊥ : Lindenbaum Q i) :=
+@[simp] lemma Lindembaum.zero_ne_succ (h : Herbrand Q i) : 0 =' Succ h = (⊥ : Lindenbaum Q i) :=
 by { induction h using fol.Herbrand.ind_on with t,
      simpa[Lindenbaum.eq_neg_of_provable_neg_0] using zero_ne_succ (Q^i) t }
 
-@[simp] lemma Lindenbaum.succ_ne_zero (h : Herbrand Q i) : Succ h ≃ 0 = (⊥ : Lindenbaum Q i) :=
+@[simp] lemma Lindenbaum.succ_ne_zero (h : Herbrand Q i) : Succ h =' 0 = (⊥ : Lindenbaum Q i) :=
 by simp [Lindenbaum.equal_symm (Succ h) 0]
 
 @[simp] lemma succ_inj (t u : term L) :
-  Q ⊢ (Succ t ≃ Succ u) ⟶ (t ≃ u) :=
-by { have : Q ⊢ ∀₁ x y, (Succ x ≃ Succ y) ⟶ (x ≃ y), by simpa[fal_fn] using provable.lextend (by_axiom robinson.q2) Q,
+  Q ⊢ (Succ t =' Succ u) ⟶ (t =' u) :=
+by { have : Q ⊢ ∀₁ x y, (Succ x =' Succ y) ⟶ (x =' y), by simpa[fal_fn] using provable.lextend (by_axiom robinson.q2) Q,
      simpa[fal_fn] using this ⊚ t ⊚ u }
 
-@[simp] lemma Lindenbaum.succ_inj  (h₁ h₂ : Herbrand Q i) : (Succ h₁ ≃ Succ h₂ : Lindenbaum Q i) = (h₁ ≃ h₂) :=
+@[simp] lemma Lindenbaum.succ_inj  (h₁ h₂ : Herbrand Q i) : (Succ h₁ =' Succ h₂ : Lindenbaum Q i) = (h₁ =' h₂) :=
 by { induction h₁ using fol.Herbrand.ind_on with t,
      induction h₂ using fol.Herbrand.ind_on with u,
-     have : Q^i ⊢ (Succ t ≃ Succ u) ⟷ (t ≃ u), by simp[iff_equiv],
+     have : Q^i ⊢ (Succ t =' Succ u) ⟷ (t =' u), by simp[iff_equiv],
      simpa using Lindenbaum.eq_of_provable_equiv.mp this }
 
 lemma Herbrand.succ_injective : function.injective (has_succ.succ : Herbrand Q i → Herbrand Q i) :=
@@ -242,29 +242,29 @@ begin
   induction h₁ using fol.Herbrand.ind_on with t,
   induction h₂ using fol.Herbrand.ind_on with u,
   intros h,
-  have lmm₁ : Q^i ⊢ Succ t ≃ Succ u, from Herbrand.eq_of_provable_equiv.mpr (by simp[h]),
-  have lmm₂ : Q^i ⊢ (Succ t ≃ Succ u) ⟶ (t ≃ u), by simp, 
-  have : Q^i ⊢ t ≃ u, from lmm₂ ⨀ lmm₁,
+  have lmm₁ : Q^i ⊢ Succ t =' Succ u, from Herbrand.eq_of_provable_equiv.mpr (by simp[h]),
+  have lmm₂ : Q^i ⊢ (Succ t =' Succ u) ⟶ (t =' u), by simp, 
+  have : Q^i ⊢ t =' u, from lmm₂ ⨀ lmm₁,
   exact Herbrand.eq_of_provable_equiv.mp this
 end
 
 @[simp] lemma Herbrand.succ_injective_iff (h₁ h₂ : Herbrand Q i) : Succ h₁ = Succ h₂ ↔ h₁ = h₂ :=
 ⟨@@Herbrand.succ_injective _ Q _ i, λ h, by simp[h]⟩
 
-@[simp] lemma zero_or_succ (t) : Q ⊢ (t ≃ 0) ⊔ (∃₁ y, t^1 ≃ Succ y) :=
-by { have : Q ⊢ ∀₁ x, (x ≃ 0) ⊔ (∃₁ y, x ≃ Succ y), by simpa[fal_fn, ex_fn] using provable.lextend (by_axiom robinson.q3) Q,
+@[simp] lemma zero_or_succ (t) : Q ⊢ (t =' 0) ⊔ (∃₁ y, t^1 =' Succ y) :=
+by { have : Q ⊢ ∀₁ x, (x =' 0) ⊔ (∃₁ y, x =' Succ y), by simpa[fal_fn, ex_fn] using provable.lextend (by_axiom robinson.q3) Q,
      simpa[fal_fn, ex_fn] using this ⊚ t }
 
-@[simp] lemma add_zero (t : term L) : Q ⊢ t + 0 ≃ t :=
-by { have : Q ⊢ ∀₁ x, (x + 0 ≃ x), by simpa[fal_fn, ex_fn] using provable.lextend (by_axiom robinson.q4) Q,
+@[simp] lemma add_zero (t : term L) : Q ⊢ t + 0 =' t :=
+by { have : Q ⊢ ∀₁ x, (x + 0 =' x), by simpa[fal_fn, ex_fn] using provable.lextend (by_axiom robinson.q4) Q,
      simpa[fal_fn, ex_fn] using this ⊚ t }
 
 @[simp] lemma Herbrand.add_zero (h : Herbrand Q i) : h + 0 = h :=
 by { induction h using fol.Herbrand.ind_on with t,
      simpa using Herbrand.eq_of_provable_equiv.mp (add_zero (Q^i) t) }
 
-@[simp] lemma add_succ (t u : term L) : Q ⊢ t + Succ u ≃ Succ (t + u) :=
-by { have : Q ⊢ ∀₁ x y, x + Succ y ≃ Succ (x + y), by simpa[fal_fn, ex_fn] using provable.lextend (by_axiom robinson.q5) Q,
+@[simp] lemma add_succ (t u : term L) : Q ⊢ t + Succ u =' Succ (t + u) :=
+by { have : Q ⊢ ∀₁ x y, x + Succ y =' Succ (x + y), by simpa[fal_fn, ex_fn] using provable.lextend (by_axiom robinson.q5) Q,
      simpa[fal_fn, ex_fn] using this ⊚ t ⊚ u }
 
 @[simp] lemma Herbrand.add_succ {i} (h₁ h₂ : Herbrand Q i) : h₁ + Succ h₂ = Succ (h₁ + h₂) :=
@@ -272,16 +272,16 @@ by { induction h₁ using fol.Herbrand.ind_on with t,
      induction h₂ using fol.Herbrand.ind_on with u,
      simpa using Herbrand.eq_of_provable_equiv.mp (add_succ (Q^i) t u) }
 
-@[simp] lemma mul_zero (t : term L) : Q ⊢ t * 0 ≃ 0 :=
-by { have : Q ⊢ ∀₁ x, x * 0 ≃ 0, by simpa[fal_fn, ex_fn] using provable.lextend (by_axiom robinson.q6) Q,
+@[simp] lemma mul_zero (t : term L) : Q ⊢ t * 0 =' 0 :=
+by { have : Q ⊢ ∀₁ x, x * 0 =' 0, by simpa[fal_fn, ex_fn] using provable.lextend (by_axiom robinson.q6) Q,
      simpa[fal_fn, ex_fn] using this ⊚ t }
 
 @[simp] lemma Herbrand.mul_zero  (h : Herbrand Q i) : h * 0 = 0 :=
 by { induction h using fol.Herbrand.ind_on with t,
      simpa using Herbrand.eq_of_provable_equiv.mp (mul_zero (Q^i) t) }
 
-@[simp] lemma mul_succ (t u : term L) : Q ⊢ t * Succ u ≃ t * u + t :=
-by { have : Q ⊢ ∀₁ x y, x * Succ y ≃ x * y + x, by simpa[fal_fn, ex_fn] using provable.lextend (by_axiom robinson.q7) Q,
+@[simp] lemma mul_succ (t u : term L) : Q ⊢ t * Succ u =' t * u + t :=
+by { have : Q ⊢ ∀₁ x y, x * Succ y =' x * y + x, by simpa[fal_fn, ex_fn] using provable.lextend (by_axiom robinson.q7) Q,
      simpa[fal_fn, ex_fn] using this ⊚ t ⊚ u }
 
 @[simp] lemma Herbrand.mul_succ {i} (h₁ h₂ : Herbrand Q i) : h₁ * Succ h₂ = h₁ * h₂ + h₁ :=
@@ -289,12 +289,12 @@ by { induction h₁ using fol.Herbrand.ind_on with t,
      induction h₂ using fol.Herbrand.ind_on with u,
      simpa using Herbrand.eq_of_provable_equiv.mp (mul_succ (Q^i) t u) }
 
-@[simp] lemma le_iff (t u : term L) : Q ⊢ (t ≼ u) ⟷ ∃. (#0 + t^1 ≃ u^1) :=
-by { have : Q ⊢ ∀₁ x y, (x ≼ y) ⟷ ∃₁ z, (z + x ≃ y), by simpa[fal_fn, ex_fn] using provable.lextend (by_axiom robinson.q8) Q,
+@[simp] lemma le_iff (t u : term L) : Q ⊢ (t ≼ u) ⟷ ∃. (#0 + t^1 =' u^1) :=
+by { have : Q ⊢ ∀₁ x y, (x ≼ y) ⟷ ∃₁ z, (z + x =' y), by simpa[fal_fn, ex_fn] using provable.lextend (by_axiom robinson.q8) Q,
      simpa[fal_fn, ex_fn, ←term.pow_rew_distrib] using this ⊚ t ⊚ u }
 
 lemma Lindenbaum.le_iff {h₁ h₂ : Herbrand Q i} :
-  (h₁ ≼ h₂ : Lindenbaum Q i) = ∃' (♯0 + h₁.pow ≃ h₂.pow : Lindenbaum Q (i + 1)) :=
+  (h₁ ≼ h₂ : Lindenbaum Q i) = ∃' (♯0 + h₁.pow =' h₂.pow : Lindenbaum Q (i + 1)) :=
 by { induction h₁ using fol.Herbrand.ind_on with t,
      induction h₂ using fol.Herbrand.ind_on with u,
      simpa[ex_fn] using Lindenbaum.eq_of_provable_equiv.mp (le_iff (Q^i) t u) }
@@ -306,9 +306,9 @@ begin
   induction e using fol.Herbrand.ind_on with u,
   induction h₁ using fol.Herbrand.ind_on with t₁,
   induction h₂ using fol.Herbrand.ind_on with t₂,
-  have lmm₁ : Q^i ⊢ ∃. (#0 + t₁^1 ≃ t₂^1),
+  have lmm₁ : Q^i ⊢ ∃. (#0 + t₁^1 =' t₂^1),
   { refine use u _, simp, refine Herbrand.eq_of_provable_equiv.mpr (by simp[h]) },
-  have lmm₂ : Q^i ⊢ (t₁ ≼ t₂) ⟷ ∃. (#0 + t₁^1 ≃ t₂^1), by simp,
+  have lmm₂ : Q^i ⊢ (t₁ ≼ t₂) ⟷ ∃. (#0 + t₁^1 =' t₂^1), by simp,
   exact Herbrand.le_iff_provable_le.mp (of_equiv lmm₁ (equiv_symm lmm₂))
 end
 
@@ -328,35 +328,35 @@ by induction n with n IH; simp[numeral, *]
 
 end Lindenbaum
 
-@[simp] lemma add_eq_zero : Q ⊢ ∀₁ x y, (x + y ≃ 0) ⟶ (x ≃ 0) ⊓ (y ≃ 0) :=
+@[simp] lemma add_eq_zero : Q ⊢ ∀₁ x y, (x + y =' 0) ⟶ (x =' 0) ⊓ (y =' 0) :=
 begin
   refine generalize (generalize _), simp[fal_fn], 
-  have lmm₁ : ⤊⤊Q ⊢ (#0 ≃ 0) ⟶ (#1 + #0 ≃ 0) ⟶ (#1 ≃ 0) ⊓ (#0 ≃ 0),
+  have lmm₁ : ⤊⤊Q ⊢ (#0 =' 0) ⟶ (#1 + #0 =' 0) ⟶ (#1 =' 0) ⊓ (#0 =' 0),
     from (deduction.mp (by simp [le_of_provable_imply_0, rew_by_axiom₁])),
-  have lmm₂ : ⤊⤊Q ⊢ (∃₁ y, #1 ≃ Succ y) ⟶ (#1 + #0 ≃ 0) ⟶ (#1 ≃ 0) ⊓ (#0 ≃ 0),
+  have lmm₂ : ⤊⤊Q ⊢ (∃₁ y, #1 =' Succ y) ⟶ (#1 + #0 =' 0) ⟶ (#1 =' 0) ⊓ (#0 =' 0),
     from imply_ex_of_fal_imply (generalize (deduction.mp (by simp [le_of_provable_imply_0, rew_by_axiom₁]))), 
   exact case_of_ax (zero_or_succ _ #0) lmm₁ lmm₂
 end
 
 @[simp] lemma Lindenbaum.add_eq_0_of_eq_0 (x y : Herbrand Q i) :
-  (x + y ≃ 0 : Lindenbaum Q i) = (x ≃ 0) ⊓ (y ≃ 0) :=
+  (x + y =' 0 : Lindenbaum Q i) = (x =' 0) ⊓ (y =' 0) :=
 begin
   induction x using fol.Herbrand.ind_on,
   induction y using fol.Herbrand.ind_on,
-  have : Q^i ⊢ (x + y ≃ 0) ⟷ (x ≃ 0) ⊓ (y ≃ 0), 
+  have : Q^i ⊢ (x + y =' 0) ⟷ (x =' 0) ⊓ (y =' 0), 
   { simp[iff_equiv],
     refine ⟨by simpa[fal_fn] using add_eq_zero (Q^i) ⊚ x ⊚ y, deduction.mp _⟩, simp,
     simp[Herbrand.eq_of_provable_equiv_0, rew_by_axiom₁, rew_by_axiom₂] },
   simpa using Lindenbaum.eq_of_provable_equiv.mp this
 end
 
-lemma mul_eq_zero : Q ⊢ ∀₁ x y, (x * y ≃ 0) ⟶ (x ≃ 0) ⊔ (y ≃ 0) :=
+lemma mul_eq_zero : Q ⊢ ∀₁ x y, (x * y =' 0) ⟶ (x =' 0) ⊔ (y =' 0) :=
 begin
   refine generalize (generalize _), simp[fal_fn], 
-  have lmm₁ : ⤊⤊Q ⊢ (#0 ≃ 0) ⟶ (#1 * #0 ≃ 0) ⟶ (#1 ≃ 0) ⊔ (#0 ≃ 0),
+  have lmm₁ : ⤊⤊Q ⊢ (#0 =' 0) ⟶ (#1 * #0 =' 0) ⟶ (#1 =' 0) ⊔ (#0 =' 0),
   { refine (deduction.mp _),
     simp[le_of_provable_imply_0, rew_by_axiom₁] },
-  have lmm₂ : ⤊⤊Q ⊢ (∃₁ y, #1 ≃ Succ y) ⟶ (#1 * #0 ≃ 0) ⟶ (#1 ≃ 0) ⊔ (#0 ≃ 0),
+  have lmm₂ : ⤊⤊Q ⊢ (∃₁ y, #1 =' Succ y) ⟶ (#1 * #0 =' 0) ⟶ (#1 =' 0) ⊔ (#0 =' 0),
   { refine imply_ex_of_fal_imply (generalize (deduction.mp _)), simp,
     simp[le_of_provable_imply_0, rew_by_axiom₁] },
   exact case_of_ax (zero_or_succ _ #0) lmm₁ lmm₂
@@ -365,7 +365,7 @@ end
 lemma zero_le : Q ⊢ ∀₁ x, 0 ≼ x :=
 begin
   refine generalize _, simp[fal_fn],
-  have : ⤊Q ⊢ (0 ≼ #0) ⟷ (∃₁ z, z + 0 ≃ #1), by simpa using (le_iff ⤊Q 0 #0), 
+  have : ⤊Q ⊢ (0 ≼ #0) ⟷ (∃₁ z, z + 0 =' #1), by simpa using (le_iff ⤊Q 0 #0), 
   refine of_equiv (use #0 (by simp)) (equiv_symm this),
 end
 
@@ -373,10 +373,10 @@ end
 by induction h using fol.Herbrand.ind_on with t;
    simpa using Herbrand.le_iff_provable_le.mp (by simpa[fal_fn] using zero_le (Q^i) ⊚ t)
 
-@[simp] lemma le_zero_equiv_eq_zero : Q ⊢ ∀₁ x, (x ≼ 0) ⟷ (x ≃ 0) :=
+@[simp] lemma le_zero_equiv_eq_zero : Q ⊢ ∀₁ x, (x ≼ 0) ⟷ (x =' 0) :=
 begin
   refine generalize _, simp[fal_fn],
-  suffices : ⤊Q ⊢ ∃. (#0 + #1 ≃ 0) ⟷ (#0 ≃ 0),
+  suffices : ⤊Q ⊢ ∃. (#0 + #1 =' 0) ⟷ (#0 =' 0),
     by simpa[Lindenbaum.eq_of_provable_equiv_0, Lindenbaum.le_iff] using this,
   simp[iff_equiv], split,
   { refine ((pnf_imply_ex_iff_fal_imply₁ _ _).mpr $ generalize _),
@@ -384,14 +384,14 @@ begin
   { refine deduction.mp (use 0 _), simp[ı, Herbrand.eq_of_provable_equiv_0, rew_by_axiom₁] }
 end
 
-@[simp] lemma Lindenbaum.le_zero_eq_eq_zero (h : Herbrand Q i) : (h ≼ 0 : Lindenbaum Q i) = (h ≃ 0) :=
+@[simp] lemma Lindenbaum.le_zero_eq_eq_zero (h : Herbrand Q i) : (h ≼ 0 : Lindenbaum Q i) = (h =' 0) :=
 by induction h using fol.Herbrand.ind_on with t;
    simpa[Lindenbaum.eq_of_provable_equiv_0] using (le_zero_equiv_eq_zero (Q^i) ⊚ t)
 
-@[simp] lemma add_numeral_eq_numeral_add (n m : ℕ) : Q ⊢ (n˙ : term L) + m˙ ≃ (n + m)˙ :=
+@[simp] lemma add_numeral_eq_numeral_add (n m : ℕ) : Q ⊢ (n˙ : term L) + m˙ =' (n + m)˙ :=
 by simp[Herbrand.eq_of_provable_equiv_0, Lindenbaum.add_numeral_eq_numeral_add]
 
-@[simp] lemma mul_numeral_eq_numeral_mul (n m : ℕ) : Q ⊢ (n˙ : term L) * m˙ ≃ (n * m)˙ :=
+@[simp] lemma mul_numeral_eq_numeral_mul (n m : ℕ) : Q ⊢ (n˙ : term L) * m˙ =' (n * m)˙ :=
 by simp[Herbrand.eq_of_provable_equiv_0, Lindenbaum.mul_numeral_eq_numeral_mul]
 
 lemma le_numeral_of_le {n m : ℕ} (h : n ≤ m) : Q ⊢ (n˙ : term L) ≼ m˙ :=
@@ -402,33 +402,33 @@ begin
   refine of_equiv (use (l˙) _) (equiv_symm $ le_iff Q (n˙) ((l + n)˙)), simp
 end
 
-lemma le_numeral_iff (n : ℕ) : Q ⊢ ∀. ((#0 ≼ n˙) ⟷ ⋁ i : fin (n+1), #0 ≃ (i : ℕ)˙) :=
+lemma le_numeral_iff (n : ℕ) : Q ⊢ ∀. ((#0 ≼ n˙) ⟷ ⋁ i : fin (n+1), #0 =' (i : ℕ)˙) :=
 begin
-  suffices : ∀ k : ℕ, Q^k ⊢ ∀. ((#0 ≼ n˙) ⟷ ⋁ i : fin (n+1), #0 ≃ (i : ℕ)˙),
+  suffices : ∀ k : ℕ, Q^k ⊢ ∀. ((#0 ≼ n˙) ⟷ ⋁ i : fin (n+1), #0 =' (i : ℕ)˙),
   { exact this 0 },
   induction n with n IH,
   { intros k, refine generalize _, simp[Lindenbaum.eq_of_provable_equiv_0], exact Lindenbaum.le_zero_eq_eq_zero _ _ _ },
   { intros k, refine generalize _,
-    simp[←Theory.sf_itr_succ, iff_equiv, -sup_disjunction], split,
-    { have zero : Q^(k + 1) ⊢ (#0 ≃ 0) ⟶ (#0 ≼ (n + 1)˙) ⟶ ⋁ (i : fin (n.succ + 1)), #0 ≃ ↑i˙,
+    simp[←Theory.sf_itr_succ, iff_equiv, -finitary.disjunction], split,
+    { have zero : Q^(k + 1) ⊢ (#0 =' 0) ⟶ (#0 ≼ (n + 1)˙) ⟶ ⋁ (i : fin (n.succ + 1)), #0 =' ↑i˙,
       { refine (deduction.mp $ deduction.mp $ imply_or_right _ _ ⨀ (rew_of_eq 0 0 (by simp) _)), 
         simp, refine disjunction_of ⟨0, by simp⟩ (by simp[numeral]) },
-      have succ : Q^(k + 1) ⊢ (∃₁ y, #1 ≃ Succ y) ⟶ (#0 ≼ (n + 1)˙) ⟶ ⋁ (i : fin (n.succ + 1)), #0 ≃ ↑i˙,
+      have succ : Q^(k + 1) ⊢ (∃₁ y, #1 =' Succ y) ⟶ (#0 ≼ (n + 1)˙) ⟶ ⋁ (i : fin (n.succ + 1)), #0 =' ↑i˙,
       { refine (imply_ex_of_fal_imply $ generalize $ deduction.mp $ rew_of_eq (Succ #0) 1 (by simp) (deduction.mp _)),
-        simp[ -sup_disjunction, ←Theory.sf_itr_succ], 
-        have : (Q^(k + 2)) +{ #1 ≃ Succ #0 } +{ Succ #0 ≼ (n + 1)˙ } ⊢ #0 ≼ n˙,
+        simp[ -finitary.disjunction, ←Theory.sf_itr_succ], 
+        have : (Q^(k + 2)) +{ #1 =' Succ #0 } +{ Succ #0 ≼ (n + 1)˙ } ⊢ #0 ≼ n˙,
           from of_equiv_p (show _ ⊢ Succ #0 ≼ (n + 1)˙, by simp) (by simp[numeral, Lindenbaum.eq_of_provable_equiv_0]), 
-        have lmm₁ : (Q^(k + 2)) +{ #1 ≃ Succ #0 } +{ Succ #0 ≼ (n + 1)˙ } ⊢ ⋁ (i : fin (n + 1)), #0 ≃ ↑i˙,
+        have lmm₁ : (Q^(k + 2)) +{ #1 =' Succ #0 } +{ Succ #0 ≼ (n + 1)˙ } ⊢ ⋁ (i : fin (n + 1)), #0 =' ↑i˙,
           from of_equiv_p this (weakening
-            (show Q^(k + 2) ⊆ (Q^(k + 2)) +{ #1 ≃ Succ #0 } +{ Succ #0 ≼ (n + 1)˙ }, by { intros p mem, refine set.subset_insert _ _ (set.subset_insert _ _ mem) })
-            (show Q^(k + 2) ⊢ (#0 ≼ n˙) ⟷ ⋁ (i : fin (n + 1)), #0 ≃ ↑i˙, by simpa using IH (k + 2) ⊚ #0)),
-        have lmm₂ : (Q^(k + 2)) +{ #1 ≃ Succ #0 } +{ Succ #0 ≼ (n + 1)˙ } ⊢ (⋁ (i : fin (n + 1)), #0 ≃ ↑i˙) ⟶ (⋁ (i : fin (n.succ + 1)), Succ #0 ≃ ↑i˙),
-        { suffices : (Q^(k + 2)) +{ #1 ≃ Succ #0 } +{ Succ #0 ≼ (n + 1)˙ } ⊢ ⋀ (i : fin (n + 1)), (#0 ≃ ↑i˙) ⟶ ⋁ (i : fin (n.succ + 1)), Succ #0 ≃ ↑i˙,
+            (show Q^(k + 2) ⊆ (Q^(k + 2)) +{ #1 =' Succ #0 } +{ Succ #0 ≼ (n + 1)˙ }, by { intros p mem, refine set.subset_insert _ _ (set.subset_insert _ _ mem) })
+            (show Q^(k + 2) ⊢ (#0 ≼ n˙) ⟷ ⋁ (i : fin (n + 1)), #0 =' ↑i˙, by simpa using IH (k + 2) ⊚ #0)),
+        have lmm₂ : (Q^(k + 2)) +{ #1 =' Succ #0 } +{ Succ #0 ≼ (n + 1)˙ } ⊢ (⋁ (i : fin (n + 1)), #0 =' ↑i˙) ⟶ (⋁ (i : fin (n.succ + 1)), Succ #0 =' ↑i˙),
+        { suffices : (Q^(k + 2)) +{ #1 =' Succ #0 } +{ Succ #0 ≼ (n + 1)˙ } ⊢ ⋀ (i : fin (n + 1)), (#0 =' ↑i˙) ⟶ ⋁ (i : fin (n.succ + 1)), Succ #0 =' ↑i˙,
             from of_equiv this (conj_imply_iff_disj_imply _ _),
-          refine conjunction_iff.mpr (λ i, deduction.mp $ rew_of_eq (↑i˙) 0 (by simp) _), simp[-sup_disjunction],
+          refine conjunction_iff.mpr (λ i, deduction.mp $ rew_of_eq (↑i˙) 0 (by simp) _), simp[-finitary.disjunction],
           refine disjunction_of ⟨i + 1, by simp⟩ (by simp[numeral]) },
         exact lmm₂ ⨀ lmm₁ },
-      exact case_of_ax (show (Q^(k + 1)) ⊢ (#0 ≃ 0) ⊔ ∃₁ y, (#1 ≃ Succ y), from zero_or_succ (Q^(k + 1)) #0) zero succ },
+      exact case_of_ax (show (Q^(k + 1)) ⊢ (#0 =' 0) ⊔ ∃₁ y, (#1 =' Succ y), from zero_or_succ (Q^(k + 1)) #0) zero succ },
     { refine of_equiv (conjunction_iff.mpr _) (conj_imply_iff_disj_imply _ _),
       rintros ⟨i, hi⟩, refine (deduction.mp $  rew_of_eq (i˙) 0 (by simp) _),
       simp[←nat.add_one],
@@ -506,13 +506,13 @@ begin
   simpa using provable.fal_complete_rew _ ı ⨀ this
 end
 
-@[simp] lemma zero_add : Iₒₚₑₙ ⊢ ∀₁ x, 0 + x ≃ x :=
+@[simp] lemma zero_add : Iₒₚₑₙ ⊢ ∀₁ x, 0 + x =' x :=
 begin
-  have lmm₁ : Iₒₚₑₙ ⊢ (0 + 0 ≃ 0) ⟶ ∀. ((0 + #0 ≃ #0) ⟶ (0 + Succ #0 ≃ Succ #0)) ⟶ ∀. (0 + #0 ≃ #0), 
-    by simpa using Ind.I_succ_induction is_open Iₒₚₑₙ (0 + #0 ≃ #0) (by simp[set.mem_def]),
-  have lmm₂ : Iₒₚₑₙ ⊢ ∀. ((0 + #0 ≃ #0) ⟶ (0 + Succ #0 ≃ Succ #0)),
+  have lmm₁ : Iₒₚₑₙ ⊢ (0 + 0 =' 0) ⟶ ∀. ((0 + #0 =' #0) ⟶ (0 + Succ #0 =' Succ #0)) ⟶ ∀. (0 + #0 =' #0), 
+    by simpa using Ind.I_succ_induction is_open Iₒₚₑₙ (0 + #0 =' #0) (by simp[set.mem_def]),
+  have lmm₂ : Iₒₚₑₙ ⊢ ∀. ((0 + #0 =' #0) ⟶ (0 + Succ #0 =' Succ #0)),
   { refine generalize (deduction.mp _), 
-    have : ⤊Iₒₚₑₙ +{ 0 + #0 ≃ #0 } ⊢ 0 + #0 ≃ #0, by simp,
+    have : ⤊Iₒₚₑₙ +{ 0 + #0 =' #0 } ⊢ 0 + #0 =' #0, by simp,
     simp[Herbrand.eq_of_provable_equiv_0] at this ⊢, exact this },
   simpa using (lmm₁ ⨀ (by simp[Herbrand.eq_of_provable_equiv_0]) ⨀ lmm₂)
 end
@@ -521,16 +521,16 @@ end
 by induction h using fol.Herbrand.ind_on with t;
    simpa using Herbrand.eq_of_provable_equiv.mp (zero_add (Iₒₚₑₙ^i) ⊚ t)
 
-@[simp] lemma succ_add : Iₒₚₑₙ ⊢ ∀₁ x y, Succ x + y ≃ Succ (x + y) :=
+@[simp] lemma succ_add : Iₒₚₑₙ ⊢ ∀₁ x y, Succ x + y =' Succ (x + y) :=
 begin
-  have ind : ⤊Iₒₚₑₙ ⊢ (Succ #0 + 0 ≃ Succ (#0 + 0)) ⟶
-                    ∀. ((Succ #1 + #0 ≃ Succ (#1 + #0)) ⟶ (Succ #1 + Succ #0 ≃ Succ (#1 + Succ #0))) ⟶
-                    ∀. (Succ #1 + #0 ≃ Succ (#1 + #0)), 
-  by simpa using Ind.I_succ_induction is_open ⤊Iₒₚₑₙ (Succ #1 + #0 ≃ Succ (#1 + #0)) (by simp[set.mem_def]),
-  have zero : ⤊Iₒₚₑₙ ⊢ Succ #0 + 0 ≃ Succ (#0 + 0),  by simp[Herbrand.eq_of_provable_equiv_0],
-  have succ : ⤊Iₒₚₑₙ ⊢ ∀. ((Succ #1 + #0 ≃ Succ (#1 + #0)) ⟶ (Succ #1 + Succ #0 ≃ Succ (#1 + Succ #0))),
+  have ind : ⤊Iₒₚₑₙ ⊢ (Succ #0 + 0 =' Succ (#0 + 0)) ⟶
+                    ∀. ((Succ #1 + #0 =' Succ (#1 + #0)) ⟶ (Succ #1 + Succ #0 =' Succ (#1 + Succ #0))) ⟶
+                    ∀. (Succ #1 + #0 =' Succ (#1 + #0)), 
+  by simpa using Ind.I_succ_induction is_open ⤊Iₒₚₑₙ (Succ #1 + #0 =' Succ (#1 + #0)) (by simp[set.mem_def]),
+  have zero : ⤊Iₒₚₑₙ ⊢ Succ #0 + 0 =' Succ (#0 + 0),  by simp[Herbrand.eq_of_provable_equiv_0],
+  have succ : ⤊Iₒₚₑₙ ⊢ ∀. ((Succ #1 + #0 =' Succ (#1 + #0)) ⟶ (Succ #1 + Succ #0 =' Succ (#1 + Succ #0))),
   { refine (generalize $ deduction.mp _), simp,
-    have : ⤊⤊Iₒₚₑₙ +{ Succ #1 + #0 ≃ Succ (#1 + #0) } ⊢ Succ #1 + #0 ≃ Succ (#1 + #0), by simp,
+    have : ⤊⤊Iₒₚₑₙ +{ Succ #1 + #0 =' Succ (#1 + #0) } ⊢ Succ #1 + #0 =' Succ (#1 + #0), by simp,
     simp[Herbrand.eq_of_provable_equiv_0] at this ⊢,  exact this },
   simpa using (generalize $ ind ⨀ zero ⨀ succ)
 end
@@ -540,14 +540,14 @@ by induction h₁ using fol.Herbrand.ind_on with t;
    induction h₂ using fol.Herbrand.ind_on with u;
    simpa using Herbrand.eq_of_provable_equiv.mp (succ_add (Iₒₚₑₙ^i) ⊚ t ⊚ u)
 
-lemma add_commutative : Iₒₚₑₙ ⊢ ∀₁ x y, x + y ≃ y + x :=
+lemma add_commutative : Iₒₚₑₙ ⊢ ∀₁ x y, x + y =' y + x :=
 begin
-  have ind : ⤊Iₒₚₑₙ ⊢ (#0 + 0 ≃ 0 + #0) ⟶ ∀. ((#1 + #0 ≃ #0 + #1) ⟶ (#1 + Succ #0 ≃ Succ #0 + #1)) ⟶ ∀. (#1 + #0 ≃ #0 + #1),
-    by simpa using Ind.I_succ_induction is_open ⤊Iₒₚₑₙ (#1 + #0 ≃ #0 + #1) (by simp[set.mem_def]),
-  have zero : ⤊Iₒₚₑₙ ⊢ #0 + 0 ≃ 0 + #0, by simp[Herbrand.eq_of_provable_equiv_0],
-  have succ : ⤊Iₒₚₑₙ ⊢ ∀. ((#1 + #0 ≃ #0 + #1) ⟶ (#1 + Succ #0 ≃ Succ #0 + #1)),
+  have ind : ⤊Iₒₚₑₙ ⊢ (#0 + 0 =' 0 + #0) ⟶ ∀. ((#1 + #0 =' #0 + #1) ⟶ (#1 + Succ #0 =' Succ #0 + #1)) ⟶ ∀. (#1 + #0 =' #0 + #1),
+    by simpa using Ind.I_succ_induction is_open ⤊Iₒₚₑₙ (#1 + #0 =' #0 + #1) (by simp[set.mem_def]),
+  have zero : ⤊Iₒₚₑₙ ⊢ #0 + 0 =' 0 + #0, by simp[Herbrand.eq_of_provable_equiv_0],
+  have succ : ⤊Iₒₚₑₙ ⊢ ∀. ((#1 + #0 =' #0 + #1) ⟶ (#1 + Succ #0 =' Succ #0 + #1)),
   { refine (generalize $ deduction.mp _), simp,
-    have : ⤊⤊Iₒₚₑₙ +{ #1 + #0 ≃ #0 + #1 } ⊢ #1 + #0 ≃ #0 + #1, by simp,
+    have : ⤊⤊Iₒₚₑₙ +{ #1 + #0 =' #0 + #1 } ⊢ #1 + #0 =' #0 + #1, by simp,
     simp[Herbrand.eq_of_provable_equiv_0] at this ⊢, exact this },
   simpa using (generalize $ ind ⨀ zero ⨀ succ)
 end
@@ -557,16 +557,16 @@ by induction h₁ using fol.Herbrand.ind_on with t;
    induction h₂ using fol.Herbrand.ind_on with u;
    simpa using Herbrand.eq_of_provable_equiv.mp (add_commutative (Iₒₚₑₙ^i) ⊚ t ⊚ u)
 
-lemma add_associative : Iₒₚₑₙ ⊢ ∀₁ x y z, x + y + z ≃ x + (y + z) :=
+lemma add_associative : Iₒₚₑₙ ⊢ ∀₁ x y z, x + y + z =' x + (y + z) :=
 begin
-  have ind : ⤊⤊Iₒₚₑₙ ⊢ (#1 + #0 + 0 ≃ #1 + (#0 + 0)) ⟶
-                     ∀. ((#2 + #1 + #0 ≃ #2 + (#1 + #0)) ⟶ (#2 + #1 + Succ #0 ≃ #2 + (#1 + Succ #0))) ⟶
-                     ∀. (#2 + #1 + #0 ≃ #2 + (#1 + #0)),
-  by simpa using Ind.I_succ_induction is_open ⤊⤊Iₒₚₑₙ (#2 + #1 + #0 ≃ #2 + (#1 + #0)) (by simp[set.mem_def]),
-  have zero : ⤊⤊Iₒₚₑₙ ⊢ #1 + #0 + 0 ≃ #1 + (#0 + 0), by simp[Herbrand.eq_of_provable_equiv_0],
-  have succ : ⤊⤊Iₒₚₑₙ ⊢ ∀. ((#2 + #1 + #0 ≃ #2 + (#1 + #0)) ⟶ (#2 + #1 + Succ #0 ≃ #2 + (#1 + Succ #0))),
+  have ind : ⤊⤊Iₒₚₑₙ ⊢ (#1 + #0 + 0 =' #1 + (#0 + 0)) ⟶
+                     ∀. ((#2 + #1 + #0 =' #2 + (#1 + #0)) ⟶ (#2 + #1 + Succ #0 =' #2 + (#1 + Succ #0))) ⟶
+                     ∀. (#2 + #1 + #0 =' #2 + (#1 + #0)),
+  by simpa using Ind.I_succ_induction is_open ⤊⤊Iₒₚₑₙ (#2 + #1 + #0 =' #2 + (#1 + #0)) (by simp[set.mem_def]),
+  have zero : ⤊⤊Iₒₚₑₙ ⊢ #1 + #0 + 0 =' #1 + (#0 + 0), by simp[Herbrand.eq_of_provable_equiv_0],
+  have succ : ⤊⤊Iₒₚₑₙ ⊢ ∀. ((#2 + #1 + #0 =' #2 + (#1 + #0)) ⟶ (#2 + #1 + Succ #0 =' #2 + (#1 + Succ #0))),
   { refine (generalize $ deduction.mp _), simp,
-    have : ⤊⤊⤊Iₒₚₑₙ +{ #2 + #1 + #0 ≃ #2 + (#1 + #0) } ⊢ #2 + #1 + #0 ≃ #2 + (#1 + #0), by simp,
+    have : ⤊⤊⤊Iₒₚₑₙ +{ #2 + #1 + #0 =' #2 + (#1 + #0) } ⊢ #2 + #1 + #0 =' #2 + (#1 + #0), by simp,
     simp[Herbrand.eq_of_provable_equiv_0] at this ⊢, exact this },
   simpa using (generalize $ generalize $ ind ⨀ zero ⨀ succ)
 end
@@ -583,14 +583,14 @@ instance Lindenbaum.add_comm_semigroup : add_comm_semigroup (Herbrand Iₒₚₑ
   add_assoc := Lindenbaum.add_associative _ _,
   add_comm := Lindenbaum.add_commutative _ _ }
 
-lemma zero_mul : Iₒₚₑₙ ⊢ ∀₁ x, 0 * x ≃ 0 :=
+lemma zero_mul : Iₒₚₑₙ ⊢ ∀₁ x, 0 * x =' 0 :=
 begin
-  have ind : Iₒₚₑₙ ⊢ (0 * 0 ≃ 0) ⟶ ∀. ((0 * #0 ≃ 0) ⟶ (0 * Succ #0 ≃ 0)) ⟶ ∀. (0 * #0 ≃ 0),
-    by simpa using Ind.I_succ_induction is_open Iₒₚₑₙ (0 * #0 ≃ 0) (by simp[set.mem_def]), 
-  have zero : Iₒₚₑₙ ⊢ 0 * 0 ≃ 0, by simp[Herbrand.eq_of_provable_equiv_0],
-  have succ : Iₒₚₑₙ ⊢ ∀. ((0 * #0 ≃ 0) ⟶ (0 * Succ #0 ≃ 0)),
+  have ind : Iₒₚₑₙ ⊢ (0 * 0 =' 0) ⟶ ∀. ((0 * #0 =' 0) ⟶ (0 * Succ #0 =' 0)) ⟶ ∀. (0 * #0 =' 0),
+    by simpa using Ind.I_succ_induction is_open Iₒₚₑₙ (0 * #0 =' 0) (by simp[set.mem_def]), 
+  have zero : Iₒₚₑₙ ⊢ 0 * 0 =' 0, by simp[Herbrand.eq_of_provable_equiv_0],
+  have succ : Iₒₚₑₙ ⊢ ∀. ((0 * #0 =' 0) ⟶ (0 * Succ #0 =' 0)),
   { refine (generalize $ deduction.mp _),
-    have : ⤊Iₒₚₑₙ +{ 0 * #0 ≃ 0 } ⊢ 0 * #0 ≃ 0, by simp,
+    have : ⤊Iₒₚₑₙ +{ 0 * #0 =' 0 } ⊢ 0 * #0 =' 0, by simp,
     simp[Herbrand.eq_of_provable_equiv_0] at this ⊢, simp[this] },
   simpa using ind ⨀ zero ⨀ succ
 end
@@ -599,18 +599,18 @@ end
 by induction h using fol.Herbrand.ind_on with t;
    simpa using Herbrand.eq_of_provable_equiv.mp (zero_mul _ ⊚ t)
 
-lemma succ_mul : Iₒₚₑₙ ⊢ ∀₁ x y, Succ x * y ≃ x * y + y :=
+lemma succ_mul : Iₒₚₑₙ ⊢ ∀₁ x y, Succ x * y =' x * y + y :=
 begin
-  have ind : ⤊Iₒₚₑₙ ⊢ (Succ #0 * 0 ≃ #0 * 0 + 0) ⟶
-                    ∀. ((Succ #1 * #0 ≃ #1 * #0 + #0) ⟶ (Succ #1 * Succ #0 ≃ #1 * Succ #0 + Succ #0)) ⟶
-                    ∀. (Succ #1 * #0 ≃ #1 * #0 + #0),
-  by simpa using Ind.I_succ_induction is_open ⤊Iₒₚₑₙ (Succ #1 * #0 ≃ #1 * #0 + #0) (by simp[set.mem_def]),
-  have zero : ⤊Iₒₚₑₙ ⊢ Succ #0 * 0 ≃ #0 * 0 + 0, by simp[Herbrand.eq_of_provable_equiv_0],
-  have succ : ⤊Iₒₚₑₙ ⊢ ∀. ((Succ #1 * #0 ≃ #1 * #0 + #0) ⟶ (Succ #1 * Succ #0 ≃ #1 * Succ #0 + Succ #0)),
+  have ind : ⤊Iₒₚₑₙ ⊢ (Succ #0 * 0 =' #0 * 0 + 0) ⟶
+                    ∀. ((Succ #1 * #0 =' #1 * #0 + #0) ⟶ (Succ #1 * Succ #0 =' #1 * Succ #0 + Succ #0)) ⟶
+                    ∀. (Succ #1 * #0 =' #1 * #0 + #0),
+  by simpa using Ind.I_succ_induction is_open ⤊Iₒₚₑₙ (Succ #1 * #0 =' #1 * #0 + #0) (by simp[set.mem_def]),
+  have zero : ⤊Iₒₚₑₙ ⊢ Succ #0 * 0 =' #0 * 0 + 0, by simp[Herbrand.eq_of_provable_equiv_0],
+  have succ : ⤊Iₒₚₑₙ ⊢ ∀. ((Succ #1 * #0 =' #1 * #0 + #0) ⟶ (Succ #1 * Succ #0 =' #1 * Succ #0 + Succ #0)),
   { refine (generalize $ deduction.mp _),
-    have : ⤊⤊Iₒₚₑₙ +{ Succ #1 * #0 ≃ #1 * #0 + #0 } ⊢ Succ #1 * #0 ≃ #1 * #0 + #0, by simp,
+    have : ⤊⤊Iₒₚₑₙ +{ Succ #1 * #0 =' #1 * #0 + #0 } ⊢ Succ #1 * #0 =' #1 * #0 + #0, by simp,
     simp[Herbrand.eq_of_provable_equiv_0] at this ⊢,
-    calc (Succ ♯1 * ♯0 + ♯1 : Herbrand (⤊⤊Iₒₚₑₙ +{ Succ #1 * #0 ≃ #1 * #0 + #0 }) 0)
+    calc (Succ ♯1 * ♯0 + ♯1 : Herbrand (⤊⤊Iₒₚₑₙ +{ Succ #1 * #0 =' #1 * #0 + #0 }) 0)
         = ♯1 * ♯0 + ♯0 + ♯1   : by rw[this]
     ... = ♯1 * ♯0 + (♯1 + ♯0) : by simp[add_assoc, add_comm]
     ... = ♯1 * ♯0 + ♯1 + ♯0   : by simp[add_assoc] },
@@ -622,14 +622,14 @@ by induction h₁ using fol.Herbrand.ind_on with t;
    induction h₂ using fol.Herbrand.ind_on with u;
    simpa using Herbrand.eq_of_provable_equiv.mp (succ_mul _ ⊚ t ⊚ u)
 
-lemma mul_commutative : Iₒₚₑₙ ⊢ ∀₁ x y, x * y ≃ y * x :=
+lemma mul_commutative : Iₒₚₑₙ ⊢ ∀₁ x y, x * y =' y * x :=
 begin
-  have ind : ⤊Iₒₚₑₙ ⊢ (#0 * 0 ≃ 0 * #0) ⟶ ∀. ((#1 * #0 ≃ #0 * #1) ⟶ (#1 * Succ #0 ≃ Succ #0 * #1)) ⟶ ∀. (#1 * #0 ≃ #0 * #1),
-    by simpa using Ind.I_succ_induction is_open ⤊Iₒₚₑₙ (#1 * #0 ≃ #0 * #1) (by simp[set.mem_def]),
-  have zero : ⤊Iₒₚₑₙ ⊢ #0 * 0 ≃ 0 * #0, by simp[Herbrand.eq_of_provable_equiv_0],
-  have succ : ⤊Iₒₚₑₙ ⊢ ∀. ((#1 * #0 ≃ #0 * #1) ⟶ (#1 * Succ #0 ≃ Succ #0 * #1)),
+  have ind : ⤊Iₒₚₑₙ ⊢ (#0 * 0 =' 0 * #0) ⟶ ∀. ((#1 * #0 =' #0 * #1) ⟶ (#1 * Succ #0 =' Succ #0 * #1)) ⟶ ∀. (#1 * #0 =' #0 * #1),
+    by simpa using Ind.I_succ_induction is_open ⤊Iₒₚₑₙ (#1 * #0 =' #0 * #1) (by simp[set.mem_def]),
+  have zero : ⤊Iₒₚₑₙ ⊢ #0 * 0 =' 0 * #0, by simp[Herbrand.eq_of_provable_equiv_0],
+  have succ : ⤊Iₒₚₑₙ ⊢ ∀. ((#1 * #0 =' #0 * #1) ⟶ (#1 * Succ #0 =' Succ #0 * #1)),
   { refine (generalize $ deduction.mp _), simp,
-    have : ⤊⤊Iₒₚₑₙ +{ #1 * #0 ≃ #0 * #1 } ⊢ #1 * #0 ≃ #0 * #1, by simp,
+    have : ⤊⤊Iₒₚₑₙ +{ #1 * #0 =' #0 * #1 } ⊢ #1 * #0 =' #0 * #1, by simp,
     simp[Herbrand.eq_of_provable_equiv_0] at this ⊢, simp[this] },
   simpa using (generalize $ ind ⨀ zero ⨀ succ)
 end
@@ -639,16 +639,16 @@ by induction h₁ using fol.Herbrand.ind_on with t;
    induction h₂ using fol.Herbrand.ind_on with u;
    simpa using Herbrand.eq_of_provable_equiv.mp (mul_commutative _ ⊚ t ⊚ u)
 
-lemma mul_add : Iₒₚₑₙ ⊢ ∀₁ x y z, x * (y + z) ≃ x * y + x * z :=
+lemma mul_add : Iₒₚₑₙ ⊢ ∀₁ x y z, x * (y + z) =' x * y + x * z :=
 begin
-  have ind : ⤊⤊Iₒₚₑₙ ⊢ (#1 * (#0 + 0) ≃ #1 * #0 + #1 * 0) ⟶
-                     ∀. ((#2 * (#1 + #0) ≃ #2 * #1 + #2 * #0) ⟶ (#2 * (#1 + Succ #0) ≃ #2 * #1 + #2 * Succ #0)) ⟶
-                     ∀. (#2 * (#1 + #0) ≃ #2 * #1 + #2 * #0),
-  by simpa using Ind.I_succ_induction is_open ⤊⤊Iₒₚₑₙ (#2 * (#1 + #0) ≃ #2 * #1 + #2 * #0) (by simp[set.mem_def]),
-  have zero : ⤊⤊Iₒₚₑₙ ⊢ #1 * (#0 + 0) ≃ #1 * #0 + #1 * 0, by simp[Herbrand.eq_of_provable_equiv_0],
-  have succ : ⤊⤊Iₒₚₑₙ ⊢ ∀. ((#2 * (#1 + #0) ≃ #2 * #1 + #2 * #0) ⟶ (#2 * (#1 + Succ #0) ≃ #2 * #1 + #2 * Succ #0)),
+  have ind : ⤊⤊Iₒₚₑₙ ⊢ (#1 * (#0 + 0) =' #1 * #0 + #1 * 0) ⟶
+                     ∀. ((#2 * (#1 + #0) =' #2 * #1 + #2 * #0) ⟶ (#2 * (#1 + Succ #0) =' #2 * #1 + #2 * Succ #0)) ⟶
+                     ∀. (#2 * (#1 + #0) =' #2 * #1 + #2 * #0),
+  by simpa using Ind.I_succ_induction is_open ⤊⤊Iₒₚₑₙ (#2 * (#1 + #0) =' #2 * #1 + #2 * #0) (by simp[set.mem_def]),
+  have zero : ⤊⤊Iₒₚₑₙ ⊢ #1 * (#0 + 0) =' #1 * #0 + #1 * 0, by simp[Herbrand.eq_of_provable_equiv_0],
+  have succ : ⤊⤊Iₒₚₑₙ ⊢ ∀. ((#2 * (#1 + #0) =' #2 * #1 + #2 * #0) ⟶ (#2 * (#1 + Succ #0) =' #2 * #1 + #2 * Succ #0)),
   { refine (generalize $ deduction.mp _), simp, 
-    have : ⤊⤊⤊Iₒₚₑₙ +{ #2 * (#1 + #0) ≃ #2 * #1 + #2 * #0 } ⊢ #2 * (#1 + #0) ≃ #2 * #1 + #2 * #0, by simp,
+    have : ⤊⤊⤊Iₒₚₑₙ +{ #2 * (#1 + #0) =' #2 * #1 + #2 * #0 } ⊢ #2 * (#1 + #0) =' #2 * #1 + #2 * #0, by simp,
     simp[Herbrand.eq_of_provable_equiv_0] at this ⊢,
     simp[this, add_assoc] },
   simpa using (generalize $ generalize $ ind ⨀ zero ⨀ succ)
@@ -660,16 +660,16 @@ by induction h₁ using fol.Herbrand.ind_on with t₁;
    induction h₃ using fol.Herbrand.ind_on with t₃;
    simpa using Herbrand.eq_of_provable_equiv.mp (mul_add _ ⊚ t₁ ⊚ t₂ ⊚ t₃)
 
-lemma mul_associative : Iₒₚₑₙ ⊢ ∀₁ x y z, x * y * z ≃ x * (y * z) :=
+lemma mul_associative : Iₒₚₑₙ ⊢ ∀₁ x y z, x * y * z =' x * (y * z) :=
 begin
-  have ind : ⤊⤊Iₒₚₑₙ ⊢ (#1 * #0 * 0 ≃ #1 * (#0 * 0)) ⟶
-                     ∀. ((#2 * #1 * #0 ≃ #2 * (#1 * #0)) ⟶ (#2 * #1 * Succ #0 ≃ #2 * (#1 * Succ #0))) ⟶
-                     ∀. (#2 * #1 * #0 ≃ #2 * (#1 * #0)),
-  by simpa using Ind.I_succ_induction is_open ⤊⤊Iₒₚₑₙ (#2 * #1 * #0 ≃ #2 * (#1 * #0)) (by simp[set.mem_def]),
-  have zero : ⤊⤊Iₒₚₑₙ ⊢ #1 * #0 * 0 ≃ #1 * (#0 * 0), by simp[Herbrand.eq_of_provable_equiv_0],
-  have succ : ⤊⤊Iₒₚₑₙ ⊢ ∀. ((#2 * #1 * #0 ≃ #2 * (#1 * #0)) ⟶ (#2 * #1 * Succ #0 ≃ #2 * (#1 * Succ #0))),
+  have ind : ⤊⤊Iₒₚₑₙ ⊢ (#1 * #0 * 0 =' #1 * (#0 * 0)) ⟶
+                     ∀. ((#2 * #1 * #0 =' #2 * (#1 * #0)) ⟶ (#2 * #1 * Succ #0 =' #2 * (#1 * Succ #0))) ⟶
+                     ∀. (#2 * #1 * #0 =' #2 * (#1 * #0)),
+  by simpa using Ind.I_succ_induction is_open ⤊⤊Iₒₚₑₙ (#2 * #1 * #0 =' #2 * (#1 * #0)) (by simp[set.mem_def]),
+  have zero : ⤊⤊Iₒₚₑₙ ⊢ #1 * #0 * 0 =' #1 * (#0 * 0), by simp[Herbrand.eq_of_provable_equiv_0],
+  have succ : ⤊⤊Iₒₚₑₙ ⊢ ∀. ((#2 * #1 * #0 =' #2 * (#1 * #0)) ⟶ (#2 * #1 * Succ #0 =' #2 * (#1 * Succ #0))),
   { refine (generalize $ deduction.mp _),
-    have : ⤊⤊⤊Iₒₚₑₙ +{ #2 * #1 * #0 ≃ #2 * (#1 * #0) } ⊢ #2 * #1 * #0 ≃ #2 * (#1 * #0), by simp,
+    have : ⤊⤊⤊Iₒₚₑₙ +{ #2 * #1 * #0 =' #2 * (#1 * #0) } ⊢ #2 * #1 * #0 =' #2 * (#1 * #0), by simp,
     simp[Herbrand.eq_of_provable_equiv_0] at this ⊢, simp[this, Lindenbaum.mul_add] },
   simpa using (generalize $ generalize $ ind ⨀ zero ⨀ succ)
 end
@@ -680,7 +680,7 @@ by induction h₁ using fol.Herbrand.ind_on with t₁;
    induction h₃ using fol.Herbrand.ind_on with t₃;
    simpa using Herbrand.eq_of_provable_equiv.mp (mul_associative _ ⊚ t₁ ⊚ t₂ ⊚ t₃)
 
-@[simp] lemma mul_one : Iₒₚₑₙ ⊢ ∀₁ x, x * 1 ≃ x := generalize (Herbrand.eq_of_provable_equiv_0.mpr (by simp[numeral_one_def]))
+@[simp] lemma mul_one : Iₒₚₑₙ ⊢ ∀₁ x, x * 1 =' x := generalize (Herbrand.eq_of_provable_equiv_0.mpr (by simp[numeral_one_def]))
 
 @[simp] lemma Lindenbaum.mul_one (h : Herbrand Iₒₚₑₙ i) : h * 1 = h := by simp[numeral_one_def]
 
@@ -694,18 +694,18 @@ instance Lindenbaum.distrib : distrib (Herbrand Iₒₚₑₙ i) :=
   left_distrib := Lindenbaum.mul_add _ _,
   right_distrib := λ a b c, by simp[mul_comm (a + b), mul_comm a, mul_comm b, Lindenbaum.mul_add] }
 
-lemma add_right_cancel : Iₒₚₑₙ ⊢ ∀₁ x y z, (x + z ≃ y + z) ⟶ (x ≃ y) :=
+lemma add_right_cancel : Iₒₚₑₙ ⊢ ∀₁ x y z, (x + z =' y + z) ⟶ (x =' y) :=
 begin
-  have ind : ⤊⤊Iₒₚₑₙ ⊢ ((#1 + 0 ≃ #0 + 0) ⟶ (#1 ≃ #0)) ⟶
-                     ∀. (((#2 + #0 ≃ #1 + #0) ⟶ (#2 ≃ #1)) ⟶ (#2 + Succ #0 ≃ #1 + Succ #0) ⟶ (#2 ≃ #1)) ⟶
-                     ∀. ((#2 + #0 ≃ #1 + #0) ⟶ (#2 ≃ #1)),
-  by simpa using Ind.I_succ_induction is_open ⤊⤊Iₒₚₑₙ ((#2 + #0 ≃ #1 + #0) ⟶ (#2 ≃ #1)) (by simp[set.mem_def]),
-  have zero : ⤊⤊Iₒₚₑₙ ⊢ (#1 + 0 ≃ #0 + 0) ⟶ (#1 ≃ #0), by simp[Lindenbaum.le_of_provable_imply_0],
-  have succ : ⤊⤊Iₒₚₑₙ ⊢ ∀. (((#2 + #0 ≃ #1 + #0) ⟶ (#2 ≃ #1)) ⟶ (#2 + Succ #0 ≃ #1 + Succ #0) ⟶ (#2 ≃ #1)),
+  have ind : ⤊⤊Iₒₚₑₙ ⊢ ((#1 + 0 =' #0 + 0) ⟶ (#1 =' #0)) ⟶
+                     ∀. (((#2 + #0 =' #1 + #0) ⟶ (#2 =' #1)) ⟶ (#2 + Succ #0 =' #1 + Succ #0) ⟶ (#2 =' #1)) ⟶
+                     ∀. ((#2 + #0 =' #1 + #0) ⟶ (#2 =' #1)),
+  by simpa using Ind.I_succ_induction is_open ⤊⤊Iₒₚₑₙ ((#2 + #0 =' #1 + #0) ⟶ (#2 =' #1)) (by simp[set.mem_def]),
+  have zero : ⤊⤊Iₒₚₑₙ ⊢ (#1 + 0 =' #0 + 0) ⟶ (#1 =' #0), by simp[Lindenbaum.le_of_provable_imply_0],
+  have succ : ⤊⤊Iₒₚₑₙ ⊢ ∀. (((#2 + #0 =' #1 + #0) ⟶ (#2 =' #1)) ⟶ (#2 + Succ #0 =' #1 + Succ #0) ⟶ (#2 =' #1)),
   { refine (generalize $ deduction.mp $ deduction.mp _), simp,
-    have : ⤊⤊⤊Iₒₚₑₙ +{ (#2 + #0 ≃ #1 + #0) ⟶ (#2 ≃ #1) } +{ #2 + Succ #0 ≃ #1 + Succ #0 } ⊢ #2 + #0 ≃ #1 + #0,
+    have : ⤊⤊⤊Iₒₚₑₙ +{ (#2 + #0 =' #1 + #0) ⟶ (#2 =' #1) } +{ #2 + Succ #0 =' #1 + Succ #0 } ⊢ #2 + #0 =' #1 + #0,
       from deduction.mpr (by simp[Lindenbaum.le_of_provable_imply_0]),
-    exact (show _ ⊢ (#2 + #0 ≃ #1 + #0) ⟶ (#2 ≃ #1), by simp) ⨀ this },
+    exact (show _ ⊢ (#2 + #0 =' #1 + #0) ⟶ (#2 =' #1), by simp) ⨀ this },
   simpa using (generalize $ generalize $ ind ⨀ zero ⨀ succ)
 end
 
@@ -714,20 +714,20 @@ lemma Herbrand.add_right_cancel (h₁ h₂ h₃ : Herbrand Iₒₚₑₙ i) : h�
   induction h₁ using fol.Herbrand.ind_on with t₁,
   induction h₂ using fol.Herbrand.ind_on with t₂,
   induction h₃ using fol.Herbrand.ind_on with t₃,
-  have lmm₁ : Iₒₚₑₙ^i ⊢ t₁ + t₃ ≃ t₂ + t₃, from Herbrand.eq_of_provable_equiv.mpr (by simp[h]),
-  have lmm₂ : Iₒₚₑₙ^i ⊢ (t₁ + t₃ ≃ t₂ + t₃) ⟶ (t₁ ≃ t₂), by simpa[fal_fn] using add_right_cancel _ ⊚ t₁ ⊚ t₂ ⊚ t₃,
+  have lmm₁ : Iₒₚₑₙ^i ⊢ t₁ + t₃ =' t₂ + t₃, from Herbrand.eq_of_provable_equiv.mpr (by simp[h]),
+  have lmm₂ : Iₒₚₑₙ^i ⊢ (t₁ + t₃ =' t₂ + t₃) ⟶ (t₁ =' t₂), by simpa[fal_fn] using add_right_cancel _ ⊚ t₁ ⊚ t₂ ⊚ t₃,
   exact Herbrand.eq_of_provable_equiv.mp (lmm₂ ⨀ lmm₁)
 end, λ h, by simp[h]⟩
 
 lemma Herbrand.add_left_cancel (h₁ h₂ h₃ : Herbrand Iₒₚₑₙ i) : h₃ + h₁ = h₃ + h₂ ↔ h₁ = h₂ :=
 by simp[add_comm h₃, Herbrand.add_right_cancel]
 
-@[simp] lemma Lindenbaum.add_right_cancel (h₁ h₂ h₃ : Herbrand Iₒₚₑₙ i) : (h₁ + h₃ ≃ h₂ + h₃ : Lindenbaum Iₒₚₑₙ i) = (h₁ ≃ h₂) :=
+@[simp] lemma Lindenbaum.add_right_cancel (h₁ h₂ h₃ : Herbrand Iₒₚₑₙ i) : (h₁ + h₃ =' h₂ + h₃ : Lindenbaum Iₒₚₑₙ i) = (h₁ =' h₂) :=
 begin
   induction h₁ using fol.Herbrand.ind_on with t₁,
   induction h₂ using fol.Herbrand.ind_on with t₂,
   induction h₃ using fol.Herbrand.ind_on with t₃,
-  have : Iₒₚₑₙ^i ⊢ (t₁ + t₃ ≃ t₂ + t₃) ⟷ (t₁ ≃ t₂),
+  have : Iₒₚₑₙ^i ⊢ (t₁ + t₃ =' t₂ + t₃) ⟷ (t₁ =' t₂),
   { simp[iff_equiv], refine ⟨by simpa[fal_fn] using add_right_cancel _ ⊚ t₁ ⊚ t₂ ⊚ t₃, deduction.mp _⟩,
   simp[Herbrand.eq_of_provable_equiv_0, Lindenbaum.rew_by_axiom₁] },
   simpa using Lindenbaum.eq_of_provable_equiv.mp this
@@ -736,14 +736,14 @@ end
 lemma add_le_add : Iₒₚₑₙ ⊢ ∀₁ x y z, (x + z ≼ y + z) ⟷ (x ≼ y) :=
 begin
   refine (generalize $ generalize $ generalize _), simp[fal_fn],
-  suffices : ⤊⤊⤊Iₒₚₑₙ ⊢ ∃. (#0 + (#3 + #1) ≃ #2 + #1) ⟷ ∃. (#0 + #3 ≃ #2),
+  suffices : ⤊⤊⤊Iₒₚₑₙ ⊢ ∃. (#0 + (#3 + #1) =' #2 + #1) ⟷ ∃. (#0 + #3 =' #2),
   { simpa[Lindenbaum.eq_top_of_provable_0, Lindenbaum.le_iff] using this },
   simp[iff_equiv], split,
   { refine (imply_ex_of_fal_imply $ generalize $ deduction.mp $ use #0 _), simp[formula.pow_eq], 
-    have : ⤊⤊⤊⤊Iₒₚₑₙ +{ #0 + (#3 + #1) ≃ #2 + #1 } ⊢ #0 + (#3 + #1) ≃ #2 + #1, by simp,
+    have : ⤊⤊⤊⤊Iₒₚₑₙ +{ #0 + (#3 + #1) =' #2 + #1 } ⊢ #0 + (#3 + #1) =' #2 + #1, by simp,
     simp[Herbrand.eq_of_provable_equiv_0, ←add_assoc, Herbrand.add_right_cancel] at this ⊢, exact this },
   { refine (imply_ex_of_fal_imply $ generalize $ deduction.mp $ use #0 _), simp[formula.pow_eq],
-    have : ⤊⤊⤊⤊Iₒₚₑₙ +{ #0 + #3 ≃ #2 } ⊢ #0 + #3 ≃ #2, by simp,
+    have : ⤊⤊⤊⤊Iₒₚₑₙ +{ #0 + #3 =' #2 } ⊢ #0 + #3 =' #2, by simp,
     simp[Herbrand.eq_of_provable_equiv_0, ←add_assoc, Herbrand.add_right_cancel] at this ⊢, exact this }
 end 
 
@@ -757,33 +757,33 @@ begin
   simpa using Lindenbaum.eq_of_provable_equiv.mp this
 end
 
-lemma lt_equiv : Iₒₚₑₙ' ⊢ ∀₁ x y, (x ≺ y) ⟷ ∃₁ z, (Succ z + x ≃ y) :=
+lemma lt_equiv : Iₒₚₑₙ' ⊢ ∀₁ x y, (x ≺ y) ⟷ ∃₁ z, (Succ z + x =' y) :=
 begin
   refine (generalize $ generalize _), simp[fal_fn, ex_fn],
-  suffices : ⤊⤊Iₒₚₑₙ' ⊢ (#1 ≼ #0) ⊓ (#1 ≄ #0) ⟷ ∃. (Succ #0 + #(1 + 1) ≃ #1),
+  suffices : ⤊⤊Iₒₚₑₙ' ⊢ (#1 ≼ #0) ⊓ (#1 ≠' #0) ⟷ ∃. (Succ #0 + #(1 + 1) =' #1),
     by simpa[lt, Lindenbaum.eq_of_provable_equiv_0, Lindenbaum.lt_eq] using this,
   simp[iff_equiv], split,
-  { suffices : ⤊⤊Iₒₚₑₙ' ⊢ (∃. (#0 + #2 ≃ #1)) ⟶ ∼(#1 ≃ #0) ⟶ ∃. (Succ #0 + #2 ≃ #1),
+  { suffices : ⤊⤊Iₒₚₑₙ' ⊢ (∃. (#0 + #2 =' #1)) ⟶ ∼(#1 =' #0) ⟶ ∃. (Succ #0 + #2 =' #1),
     { simp[Lindenbaum.le_of_provable_imply_0, Lindenbaum.le_iff] at this ⊢,
       simpa[sdiff_eq] using sdiff_le_iff.mpr (by simpa[sdiff_eq] using this) },
     refine (imply_ex_of_fal_imply $ generalize $ deduction.mp $ rew_of_eq (#0 + #2) 1 (eq_symm $ by simp) _),
     simp[formula.pow_eq],
-    have zero : ⤊⤊⤊Iₒₚₑₙ' +{ #0 + #2 ≃ #1 } ⊢ (#0 ≃ 0) ⟶ (#2 ≄ #0 + #2) ⟶ ∃. (Succ #0 + #3 ≃ #1 + #3),
+    have zero : ⤊⤊⤊Iₒₚₑₙ' +{ #0 + #2 =' #1 } ⊢ (#0 =' 0) ⟶ (#2 ≠' #0 + #2) ⟶ ∃. (Succ #0 + #3 =' #1 + #3),
     { refine (deduction.mp _), simp[Lindenbaum.le_of_provable_imply_0, Lindenbaum.rew_by_axiom₁] },
-    have succ : ⤊⤊⤊Iₒₚₑₙ' +{ #0 + #2 ≃ #1 } ⊢ (∃₁ y, #1 ≃ Succ y) ⟶ (#2 ≄ #0 + #2) ⟶ ∃. (Succ #0 + #3 ≃ #1 + #3),
+    have succ : ⤊⤊⤊Iₒₚₑₙ' +{ #0 + #2 =' #1 } ⊢ (∃₁ y, #1 =' Succ y) ⟶ (#2 ≠' #0 + #2) ⟶ ∃. (Succ #0 + #3 =' #1 + #3),
     { refine (imply_ex_of_fal_imply $ generalize $ deduction.mp $ deduction.mp $ use #0 _), simp[←sf_dsb], 
       simp[Herbrand.eq_of_provable_equiv_0, Lindenbaum.rew_by_axiom₂] },
     exact case_of_ax (zero_or_succ _ #0) zero succ },
   { refine (imply_ex_of_fal_imply $ generalize $ deduction.mp $ rew_of_eq (Succ #0 + #2) 1 (eq_symm $ by simp) _), simp,
     simp[Herbrand.le_iff_provable_le_0, Lindenbaum.eq_neg_of_provable_neg_0, -Lindenbaum.succ_add],
-    simpa using Lindenbaum.add_right_cancel (⤊⤊⤊Iₒₚₑₙ' +{ Succ #0 + #2 ≃ #1 }) 0 0 (Succ ♯0) ♯2, }
+    simpa using Lindenbaum.add_right_cancel (⤊⤊⤊Iₒₚₑₙ' +{ Succ #0 + #2 =' #1 }) 0 0 (Succ ♯0) ♯2, }
 end
 
-lemma lt_equiv' (x y) : Iₒₚₑₙ' ⊢ (x ≺ y) ⟷ ∃₁ z, (Succ z + x^1 ≃ y^1) :=
+lemma lt_equiv' (x y) : Iₒₚₑₙ' ⊢ (x ≺ y) ⟷ ∃₁ z, (Succ z + x^1 =' y^1) :=
 by simpa[lt, fal_fn, ex_fn, ←term.pow_rew_distrib] using (lt_equiv _) ⊚ x ⊚ y 
 
 lemma Lindenbaum.lt_eq (h₁ h₂ : Herbrand Iₒₚₑₙ' i) :
-  (h₁ ≺' h₂) = ∃' (Succ ♯0 + h₁.pow ≃ h₂.pow : Lindenbaum Iₒₚₑₙ' (i + 1)) :=
+  (h₁ ≺' h₂) = ∃' (Succ ♯0 + h₁.pow =' h₂.pow : Lindenbaum Iₒₚₑₙ' (i + 1)) :=
 by induction h₁ using fol.Herbrand.ind_on with t;
    induction h₂ using fol.Herbrand.ind_on with u;
    simpa[lt, fal_fn, ex_fn] using Lindenbaum.eq_of_provable_equiv.mp ((lt_equiv' (Iₒₚₑₙ'^i) t u))
@@ -799,11 +799,11 @@ by { have : h ≤ 1 + h, from robinson.Lindenbaum.le_add_self Iₒₚₑₙ i h 
 lemma le_transitive : Iₒₚₑₙ ⊢ ∀₁ x y z, (x ≼ y) ⟶ (y ≼ z) ⟶ (x ≼ z) :=
 begin
   refine (generalize $ generalize $ generalize _), simp[fal_fn],
-  suffices : ⤊⤊⤊Iₒₚₑₙ ⊢ ∃. (#0 + #3 ≃ #2) ⟶ ∃. (#0 + #2 ≃ #1) ⟶ ∃. (#0 + #3 ≃ #1),
+  suffices : ⤊⤊⤊Iₒₚₑₙ ⊢ ∃. (#0 + #3 =' #2) ⟶ ∃. (#0 + #2 =' #1) ⟶ ∃. (#0 + #3 =' #1),
   { simp[Lindenbaum.eq_top_of_provable_0, Lindenbaum.le_iff] at this ⊢, exact this },
   refine (imply_ex_of_fal_imply $ generalize $ deduction.mp $ imply_ex_of_fal_imply $ generalize $ deduction.mp $ use (#0 + #1) _),
   simp[←sf_dsb, formula.pow_eq],
-  show (Iₒₚₑₙ^5) +{ #1 + #4 ≃ #3 } +{ #0 + #3 ≃ #2 } ⊢ #0 + #1 + #4 ≃ #2,
+  show (Iₒₚₑₙ^5) +{ #1 + #4 =' #3 } +{ #0 + #3 =' #2 } ⊢ #0 + #1 + #4 =' #2,
   by simp[Herbrand.eq_of_provable_equiv_0, Lindenbaum.rew_by_axiom₁_inv, Lindenbaum.rew_by_axiom₂_inv, add_assoc]
 end
 
@@ -822,29 +822,29 @@ lemma add_lt_of_lt_of_lt : Iₒₚₑₙ' ⊢ ∀₁ x y z v, (x ≺ y) ⟶ (z �
 begin
   refine (generalize $ generalize $ generalize $ generalize _), simp[fal_fn],
   show Iₒₚₑₙ'^4 ⊢ (#3 ≺ #2) ⟶ (#1 ≺ #0) ⟶ (#3 + #1 ≺ #2 + #0),
-  suffices : Iₒₚₑₙ'^4 ⊢ ∃. (Succ #0 + #4 ≃ #3) ⟶ ∃. (Succ #0 + #2 ≃ #1) ⟶ ∃. (Succ #0 + #4 + #2 ≃ #3 + #1),
+  suffices : Iₒₚₑₙ'^4 ⊢ ∃. (Succ #0 + #4 =' #3) ⟶ ∃. (Succ #0 + #2 =' #1) ⟶ ∃. (Succ #0 + #4 + #2 =' #3 + #1),
   { simp[lt, Lindenbaum.eq_top_of_provable_0, Lindenbaum.lt_eq, add_pow, add_assoc] at this ⊢, simpa using this },
   refine (imply_ex_of_fal_imply $ generalize $ deduction.mp $ imply_ex_of_fal_imply $ generalize $ deduction.mp $ use (Succ #1 + #0) _),
   simp[←sf_dsb, formula.pow_eq],
-  show (Iₒₚₑₙ'^6)+{ Succ #1 + #5 ≃ #4 }+{ Succ #0 + #3 ≃ #2 } ⊢ Succ (Succ #1 + #0) + #5 + #3 ≃ #4 + #2,
+  show (Iₒₚₑₙ'^6)+{ Succ #1 + #5 =' #4 }+{ Succ #0 + #3 =' #2 } ⊢ Succ (Succ #1 + #0) + #5 + #3 =' #4 + #2,
   simp[Herbrand.eq_of_provable_equiv_0, rew_by_axiom₁_inv, rew_by_axiom₂_inv],
-  calc    (♯1 + ♯0 + ♯5 + ♯3 : Herbrand ((Iₒₚₑₙ'^6)+{ Succ #1 + #5 ≃ #4 }+{ Succ #0 + #3 ≃ #2 }) 0) 
+  calc    (♯1 + ♯0 + ♯5 + ♯3 : Herbrand ((Iₒₚₑₙ'^6)+{ Succ #1 + #5 =' #4 }+{ Succ #0 + #3 =' #2 }) 0) 
         = (♯1 + (♯0 + ♯5) + ♯3) : by simp[add_assoc]
     ... = (♯1 + (♯5 + ♯0) + ♯3) : by simp[add_comm]
     ... = ♯1 + ♯5 + (♯0 + ♯3)   : by simp[add_assoc]
 end
 
-lemma eq_or_succ_le_of_le : Iₒₚₑₙ ⊢ ∀₁ x y, (x ≼ y) ⟶ (x ≃ y) ⊔ (Succ x ≼ y) :=
+lemma eq_or_succ_le_of_le : Iₒₚₑₙ ⊢ ∀₁ x y, (x ≼ y) ⟶ (x =' y) ⊔ (Succ x ≼ y) :=
 begin
   refine (generalize $ generalize _), simp[fal_fn],
-  suffices : ⤊⤊Iₒₚₑₙ ⊢ ∃. (#0 + #2 ≃ #1) ⟶ (#1 ≃ #0) ⊔ ∃. (#0 + Succ #2 ≃ #1),
+  suffices : ⤊⤊Iₒₚₑₙ ⊢ ∃. (#0 + #2 =' #1) ⟶ (#1 =' #0) ⊔ ∃. (#0 + Succ #2 =' #1),
   { simp[Lindenbaum.eq_top_of_provable_0, Lindenbaum.le_iff] at this ⊢, exact this },
   refine (imply_ex_of_fal_imply $ generalize _), simp[formula.pow_eq],
-  show Iₒₚₑₙ^3 ⊢ (#0 + #2 ≃ #1) ⟶ (#2 ≃ #1) ⊔ ∃. (#0 + Succ #3 ≃ #2),
-  have zero : Iₒₚₑₙ^3 ⊢ (#0 ≃ 0) ⟶ (#0 + #2 ≃ #1) ⟶ (#2 ≃ #1) ⊔ ∃. (#0 + Succ #3 ≃ #2),
+  show Iₒₚₑₙ^3 ⊢ (#0 + #2 =' #1) ⟶ (#2 =' #1) ⊔ ∃. (#0 + Succ #3 =' #2),
+  have zero : Iₒₚₑₙ^3 ⊢ (#0 =' 0) ⟶ (#0 + #2 =' #1) ⟶ (#2 =' #1) ⊔ ∃. (#0 + Succ #3 =' #2),
   { refine (deduction.mp $ deduction.mp _),
     simp[Lindenbaum.eq_top_of_provable_0, Lindenbaum.rew_by_axiom₁_inv, Lindenbaum.rew_by_axiom₂] },
-  have succ : Iₒₚₑₙ^3 ⊢ (∃₁ y, #1 ≃ Succ y) ⟶ (#0 + #2 ≃ #1) ⟶ (#2 ≃ #1) ⊔ ∃. (#0 + Succ #3 ≃ #2),
+  have succ : Iₒₚₑₙ^3 ⊢ (∃₁ y, #1 =' Succ y) ⟶ (#0 + #2 =' #1) ⟶ (#2 =' #1) ⊔ ∃. (#0 + Succ #3 =' #2),
   { refine (imply_ex_of_fal_imply $ generalize $ deduction.mp $ deduction.mp $ imply_or_right _ _ ⨀ use #0 _),
     simp[Lindenbaum.eq_top_of_provable_0, Lindenbaum.rew_by_axiom₁_inv, Lindenbaum.rew_by_axiom₂] },
   exact case_of_ax (zero_or_succ _ #0) zero succ
@@ -866,12 +866,12 @@ begin
       refine Lindenbaum.le_transitive _ _ this (by simp) },
     have orr : Iₒₚₑₙ^2 ⊢ (#0 ≼ #1) ⟶ (#1 ≼ Succ #0) ⊔ (Succ #0 ≼ #1),
     { refine (deduction.mp _),
-      have eq      : (Iₒₚₑₙ^2) +{ #0 ≼ #1 } ⊢ (#0 ≃ #1) ⟶ (#1 ≼ Succ #0) ⊔ (Succ #0 ≼ #1),
+      have eq      : (Iₒₚₑₙ^2) +{ #0 ≼ #1 } ⊢ (#0 =' #1) ⟶ (#1 ≼ Succ #0) ⊔ (Succ #0 ≼ #1),
       { refine (deduction.mp $ imply_or_left _ _ ⨀ _), simp[Herbrand.le_iff_provable_le_0, rew_by_axiom₁] },
       have succ_le : (Iₒₚₑₙ^2) +{ #0 ≼ #1 } ⊢ (Succ #0 ≼ #1) ⟶ (#1 ≼ Succ #0) ⊔ (Succ #0 ≼ #1),
         by simp[Lindenbaum.le_of_provable_imply_0],
-      have : (Iₒₚₑₙ^2) +{ #0 ≼ #1 } ⊢ (#0 ≃ #1) ⊔ (Succ #0 ≼ #1), 
-        from deduction.mpr (show (Iₒₚₑₙ^2) ⊢ (#0 ≼ #1) ⟶ (#0 ≃ #1) ⊔ (Succ #0 ≼ #1),
+      have : (Iₒₚₑₙ^2) +{ #0 ≼ #1 } ⊢ (#0 =' #1) ⊔ (Succ #0 ≼ #1), 
+        from deduction.mpr (show (Iₒₚₑₙ^2) ⊢ (#0 ≼ #1) ⟶ (#0 =' #1) ⊔ (Succ #0 ≼ #1),
         by simpa[fal_fn] using eq_or_succ_le_of_le _ ⊚ #0 ⊚ #1),
       exact case_of_ax this eq succ_le },
     exact or_imply _ _ _ ⨀ orl ⨀ orr },
@@ -884,28 +884,28 @@ by { have : ((coe : LA'.pr 2 → LA'.pr 2) (sum.inr additional_pr.lt)) = sum.inr
      simp[lt, this] }
 
 lemma lt_mul_of_nonzero_of_lt :
-  Iₒₚₑₙ' ⊢ ∀₁ x y z, (x ≺ y) ⟶ (z ≄ 0) ⟶ (x * z ≺ y * z) :=
+  Iₒₚₑₙ' ⊢ ∀₁ x y z, (x ≺ y) ⟶ (z ≠' 0) ⟶ (x * z ≺ y * z) :=
 begin
   have ind : Iₒₚₑₙ'^2 ⊢
-       ((#1 ≺ #0) ⟶ ((0 : term LA) ≄ 0) ⟶ (#1 * 0 ≺ #0 * 0)) ⟶
-    ∀. (((#2 ≺ #1) ⟶ (#0 ≄ 0) ⟶ (#2 * #0 ≺ #1 * #0)) ⟶ (#2 ≺ #1) ⟶ (Succ #0 ≄ 0) ⟶ (#2 * Succ #0 ≺ #1 * Succ #0)) ⟶
-    ∀. ((#2 ≺ #1) ⟶ (#0 ≄ 0) ⟶ (#2 * #0 ≺ #1 * #0)),
+       ((#1 ≺ #0) ⟶ ((0 : term LA) ≠' 0) ⟶ (#1 * 0 ≺ #0 * 0)) ⟶
+    ∀. (((#2 ≺ #1) ⟶ (#0 ≠' 0) ⟶ (#2 * #0 ≺ #1 * #0)) ⟶ (#2 ≺ #1) ⟶ (Succ #0 ≠' 0) ⟶ (#2 * Succ #0 ≺ #1 * Succ #0)) ⟶
+    ∀. ((#2 ≺ #1) ⟶ (#0 ≠' 0) ⟶ (#2 * #0 ≺ #1 * #0)),
   by simpa[additional.lt] using
-    I_succ_induction_LA (Iₒₚₑₙ'^2) ((#2 ≺ #1) ⟶ (#0 ≄ 0) ⟶ (#2 * #0 ≺ #1 * #0)) (by simp),
-  have zero : Iₒₚₑₙ'^2 ⊢ (#1 ≺ #0) ⟶ ((0 : term LA) ≄ 0) ⟶ (#1 * 0 ≺ #0 * 0), by simp[Lindenbaum.eq_top_of_provable_0],
-  have succ : Iₒₚₑₙ'^2 ⊢ ∀. (((#2 ≺ #1) ⟶ (#0 ≄ 0) ⟶ (#2 * #0 ≺ #1 * #0)) ⟶ (#2 ≺ #1) ⟶ (Succ #0 ≄ 0) ⟶ (#2 * Succ #0 ≺ #1 * Succ #0)),
+    I_succ_induction_LA (Iₒₚₑₙ'^2) ((#2 ≺ #1) ⟶ (#0 ≠' 0) ⟶ (#2 * #0 ≺ #1 * #0)) (by simp),
+  have zero : Iₒₚₑₙ'^2 ⊢ (#1 ≺ #0) ⟶ ((0 : term LA) ≠' 0) ⟶ (#1 * 0 ≺ #0 * 0), by simp[Lindenbaum.eq_top_of_provable_0],
+  have succ : Iₒₚₑₙ'^2 ⊢ ∀. (((#2 ≺ #1) ⟶ (#0 ≠' 0) ⟶ (#2 * #0 ≺ #1 * #0)) ⟶ (#2 ≺ #1) ⟶ (Succ #0 ≠' 0) ⟶ (#2 * Succ #0 ≺ #1 * Succ #0)),
   { refine (generalize $ deduction.mp $ deduction.mp $ deduction.mp _), simp[-iff_and],
-    have zero : (Iₒₚₑₙ'^3) +{ (#2 ≺ #1) ⟶ (#0 ≄ 0) ⟶ (#2 * #0 ≺ #1 * #0) } +{ #2 ≺ #1 } +{ Succ #0 ≄ 0 } ⊢ (#0 ≃ 0) ⟶ (#2 * Succ #0 ≺ #1 * Succ #0),
+    have zero : (Iₒₚₑₙ'^3) +{ (#2 ≺ #1) ⟶ (#0 ≠' 0) ⟶ (#2 * #0 ≺ #1 * #0) } +{ #2 ≺ #1 } +{ Succ #0 ≠' 0 } ⊢ (#0 =' 0) ⟶ (#2 * Succ #0 ≺ #1 * Succ #0),
     { refine (deduction.mp $ rew_of_eq 0 0 (by simp) _),
-      have : (Iₒₚₑₙ'^3) +{ (#2 ≺ #1) ⟶ (#0 ≄ 0) ⟶ (#2 * #0 ≺ #1 * #0) } +{ #2 ≺ #1 } +{ Succ #0 ≄ 0 }+{ #0 ≃ 0 } ⊢ #2 ≺ #1, by simp,
+      have : (Iₒₚₑₙ'^3) +{ (#2 ≺ #1) ⟶ (#0 ≠' 0) ⟶ (#2 * #0 ≺ #1 * #0) } +{ #2 ≺ #1 } +{ Succ #0 ≠' 0 }+{ #0 =' 0 } ⊢ #2 ≺ #1, by simp,
       simpa[Herbrand.iff_abberavation₂_0] using this },
-    have nonzero : (Iₒₚₑₙ'^3) +{ (#2 ≺ #1) ⟶ (#0 ≄ 0) ⟶ (#2 * #0 ≺ #1 * #0) } +{ #2 ≺ #1 } +{ Succ #0 ≄ 0 } ⊢ (#0 ≄ 0) ⟶ (#2 * Succ #0 ≺ #1 * Succ #0),
+    have nonzero : (Iₒₚₑₙ'^3) +{ (#2 ≺ #1) ⟶ (#0 ≠' 0) ⟶ (#2 * #0 ≺ #1 * #0) } +{ #2 ≺ #1 } +{ Succ #0 ≠' 0 } ⊢ (#0 ≠' 0) ⟶ (#2 * Succ #0 ≺ #1 * Succ #0),
     { refine (deduction.mp _),
-      have lt : (Iₒₚₑₙ'^3) +{ (#2 ≺ #1) ⟶ (#0 ≄ 0) ⟶ (#2 * #0 ≺ #1 * #0) } +{ #2 ≺ #1 } +{ Succ #0 ≄ 0 } +{ #0 ≄ 0 } ⊢ #2 * #0 ≺ #1 * #0,
-        from (show _ ⊢ (#2 ≺ #1) ⟶ (#0 ≄ 0) ⟶ (#2 * #0 ≺ #1 * #0), by simp) ⨀ (by simp) ⨀ (by simp),
+      have lt : (Iₒₚₑₙ'^3) +{ (#2 ≺ #1) ⟶ (#0 ≠' 0) ⟶ (#2 * #0 ≺ #1 * #0) } +{ #2 ≺ #1 } +{ Succ #0 ≠' 0 } +{ #0 ≠' 0 } ⊢ #2 * #0 ≺ #1 * #0,
+        from (show _ ⊢ (#2 ≺ #1) ⟶ (#0 ≠' 0) ⟶ (#2 * #0 ≺ #1 * #0), by simp) ⨀ (by simp) ⨀ (by simp),
       have : (Iₒₚₑₙ'^3) ⊢ (#2 * #0 ≺ #1 * #0) ⟶ (#2 ≺ #1) ⟶ (#2 * #0 + #2 ≺ #1 * #0 + #1),
       by simpa[fal_fn] using ((add_lt_of_lt_of_lt (Iₒₚₑₙ'^3)) ⊚ (#2 * #0) ⊚ (#1 * #0) ⊚ #2 ⊚ #1),
-      have : (Iₒₚₑₙ'^3) +{ (#2 ≺ #1) ⟶ (#0 ≄ 0) ⟶ (#2 * #0 ≺ #1 * #0) } +{ #2 ≺ #1 } +{ Succ #0 ≄ 0 } +{ #0 ≄ 0 } ⊢ #2 * #0 + #2 ≺ #1 * #0 + #1,
+      have : (Iₒₚₑₙ'^3) +{ (#2 ≺ #1) ⟶ (#0 ≠' 0) ⟶ (#2 * #0 ≺ #1 * #0) } +{ #2 ≺ #1 } +{ Succ #0 ≠' 0 } +{ #0 ≠' 0 } ⊢ #2 * #0 + #2 ≺ #1 * #0 + #1,
         from this.extend ⨀ lt ⨀ (by simp),
       simp[Lindenbaum.eq_top_of_provable_0] at this ⊢, exact this },
     refine cases_of _ _ zero nonzero },
@@ -913,23 +913,23 @@ begin
 end
 
 #check 0  /-
-lemma mul_right_cancel_of_nonzero_aux : Iₒₚₑₙ' ⊢ ∀₁ x y z, (z ≄ 0) ⟶ (x * z ≃ y * z) ⟶ (x ≃ y) :=
+lemma mul_right_cancel_of_nonzero_aux : Iₒₚₑₙ' ⊢ ∀₁ x y z, (z ≠' 0) ⟶ (x * z =' y * z) ⟶ (x =' y) :=
 begin
   refine (generalize $ generalize $ generalize _), simp[fal_fn],
-  suffices : Iₒₚₑₙ'^3 ⊢ (#0 ≄ 0) ⟶ (#2 ≄ #1) ⟶ (#2 * #0 ≄ #1 * #0),
+  suffices : Iₒₚₑₙ'^3 ⊢ (#0 ≠' 0) ⟶ (#2 ≠' #1) ⟶ (#2 * #0 ≠' #1 * #0),
   {  simp[Lindenbaum.eq_top_of_provable_0] at this ⊢, simpa[sup_comm] using this },
-  have : Iₒₚₑₙ'^3 ⊢ ∀₁ x y z, (x ≺ y) ⟶ (z ≄ 0) ⟶ (x * z ≺ y * z),
+  have : Iₒₚₑₙ'^3 ⊢ ∀₁ x y z, (x ≺ y) ⟶ (z ≠' 0) ⟶ (x * z ≺ y * z),
   have := (lt_mul_of_nonzero_of_lt (Iₒₚₑₙ'^3)),
 
   simp[fal_fn] at this,
-  have orl : Iₒₚₑₙ' ⊢ (#1 ≼ #2) ⟶ ∼(#0 ≃ 0) ⟶ ∼(#2 ≃ #1) ⟶ ∼(#2 * #0 ≃ #1 * #0),
+  have orl : Iₒₚₑₙ' ⊢ (#1 ≼ #2) ⟶ ∼(#0 =' 0) ⟶ ∼(#2 =' #1) ⟶ ∼(#2 * #0 =' #1 * #0),
   { refine (deduction.mp $ deduction.mp $ deduction.mp $ ne_symm _),
-    have : Iₒₚₑₙ' +{ #1 ≼ #2 } +{ #0 ≄ 0 } +{ #2 ≄ #1 } ⊢ _, { have h := (this ⊚ #1 ⊚ #2 ⊚ #0),  }, 
+    have : Iₒₚₑₙ' +{ #1 ≼ #2 } +{ #0 ≠' 0 } +{ #2 ≠' #1 } ⊢ _, { have h := (this ⊚ #1 ⊚ #2 ⊚ #0),  }, 
     have := this ⨀ (by {simp[lessthan_def, fal_fn], refine ne_symm (by simp) }) ⨀ (by simp[fal_fn]),
     simp[lessthan_def, fal_fn] at this, exact this.2 },
-  have orr : Iₒₚₑₙ ⊢ (#2 ≼ #1) ⟶ ∼(#0 ≃ 0) ⟶ ∼(#2 ≃ #1) ⟶ ∼(#2 * #0 ≃ #1 * #0),
+  have orr : Iₒₚₑₙ ⊢ (#2 ≼ #1) ⟶ ∼(#0 =' 0) ⟶ ∼(#2 =' #1) ⟶ ∼(#2 * #0 =' #1 * #0),
   { refine (deduction.mp $ deduction.mp $ deduction.mp _),
-    have : Iₒₚₑₙ +{ #2 ≼ #1 } +{ #0 ≄ 0 } +{ #2 ≄ #1 } ⊢ _, from provable.extend (this ⊚ #2 ⊚ #1 ⊚ #0), 
+    have : Iₒₚₑₙ +{ #2 ≼ #1 } +{ #0 ≠' 0 } +{ #2 ≠' #1 } ⊢ _, from provable.extend (this ⊚ #2 ⊚ #1 ⊚ #0), 
     have := this ⨀ (by simp[lessthan_def, fal_fn]) ⨀ (by simp[fal_fn]),
     simp[lessthan_def, fal_fn] at this, exact this.2 },
   refine case_of_ax (show Iₒₚₑₙ ⊢ (#1 ≼ #2) ⊔ (#2 ≼ #1), by simpa[fal_fn] using le_or_ge ⊚ #1 ⊚ #2) orl orr
@@ -963,7 +963,7 @@ begin
     imply_ex_of_fal_imply $ generalize $ deduction.mp $
     imply_ex_of_fal_imply $ generalize $ deduction.mp $ use (#0 * #1) _),
   simp[formula.pow_eq, ←sf_dsb],
-  show Iₒₚₑₙ +{ #1 * #5 ≃ #4 } +{ #0 * #4 ≃ #3 } ⊢ #0 * #1 * #5 ≃ #3,
+  show Iₒₚₑₙ +{ #1 * #5 =' #4 } +{ #0 * #4 =' #3 } ⊢ #0 * #1 * #5 =' #3,
   simp[Herbrand.eq_of_provable_equiv_0, rew_by_axiom₁_inv, rew_by_axiom₂_inv, mul_assoc]
 end
 -/
@@ -972,14 +972,14 @@ end Iopen
 def 
 
 
-lemma add_symm : Iₒₚₑₙ ⊢ ∀₁ x y, (x + y ≃ y + x) :=
+lemma add_symm : Iₒₚₑₙ ⊢ ∀₁ x y, (x + y =' y + x) :=
 begin
   refine (generalize _), simp[fal_fn],
-  have zero : Iₒₚₑₙ ⊢ (#0 ≃ 0) ⟶ ∀. (#1 + #0 ≃ #0 + #1),
+  have zero : Iₒₚₑₙ ⊢ (#0 =' 0) ⟶ ∀. (#1 + #0 =' #0 + #1),
   { refine (deduction.mp $ generalize _), simp[←sf_dsb, Herbrand.eq_of_provable_equiv_0, rew_by_axiom₁] },
-  have succ : Iₒₚₑₙ ⊢ (∃₁ y, #1 ≃ Succ y) ⟶ ∀. (#1 + #0 ≃ #0 + #1),
+  have succ : Iₒₚₑₙ ⊢ (∃₁ y, #1 =' Succ y) ⟶ ∀. (#1 + #0 =' #0 + #1),
   { refine (imply_ex_of_fal_imply $ generalize $ deduction.mp $ rew_of_eq (Succ #0) 1 (by simp) $ generalize _), simp[formula.pow_eq, ←sf_dsb],
-    suffices : Iₒₚₑₙ ⊢ Succ #1 + #0 ≃ #0 + Succ #1, by simp[this],
+    suffices : Iₒₚₑₙ ⊢ Succ #1 + #0 =' #0 + Succ #1, by simp[this],
      
      }
 end
