src/FOL/fol.lean
@@ -126,7 +126,7 @@ def formula_to_string [has_to_string (term L)] [∀ n, has_to_string (L.pr n)] :
 | (@formula.app _ 2 p v) := has_to_string.to_string (v 0) ++ has_to_string.to_string p ++ has_to_string.to_string (v 1)
 | (@formula.app _ (n + 3) p v) :=
     has_to_string.to_string p ++ "(" ++ @has_to_string.to_string (finitary _ _) _ v ++ ")"
-| (t ≃ u) := has_to_string.to_string t ++ " = " ++ has_to_string.to_string u
+| (t =' u) := has_to_string.to_string t ++ " = " ++ has_to_string.to_string u
 | (p ⟶ q) := formula_to_string p ++ " → " ++ formula_to_string q
 | (∼p) := "¬(" ++ formula_to_string p ++ ")"
 | (∀.p) := "∀(" ++ formula_to_string p ++ ")"
@@ -135,11 +135,11 @@ instance [has_to_string (term L)] [∀ n, has_to_string (L.pr n)] : has_to_strin
 
 @[simp] lemma formula.top_eq : @formula.verum L = (⊤) := rfl
 @[simp] lemma formula.imply_eq : @formula.imply L = (⟶) := rfl
-@[simp] lemma formula.equal_eq : @formula.equal L = (≃) := rfl
+@[simp] lemma formula.equal_eq : @formula.equal L = (=') := rfl
 @[simp] lemma formula.neg_eq : @formula.neg L = has_negation.neg := rfl
 @[simp] lemma formula.fal_eq : @formula.fal L = has_univ_quantifier.univ := rfl
 
-instance : inhabited (formula L) := ⟨(#0 : term L) ≃ #0⟩
+instance : inhabited (formula L) := ⟨(#0 : term L) =' #0⟩
 
 @[reducible] def Theory (L : language.{u}) := logic.Theory (formula L)
 
@@ -151,8 +151,8 @@ instance : has_exists_quantifier (formula L) := ⟨formula.ex⟩
 
 lemma formula.ex_eq (p : formula L) : (∃. p) = ∼∀.∼p := rfl
 
-@[simp] lemma formula.equal.inj' (t₁ u₁ t₂ u₂ : term L) : (t₁ ≃ t₂ : formula L) = (u₁ ≃ u₂) ↔ t₁ = u₁ ∧ t₂ = u₂ :=
-⟨formula.equal.inj, by simp; exact congr_arg2 (≃)⟩
+@[simp] lemma formula.equal.inj' (t₁ u₁ t₂ u₂ : term L) : (t₁ =' t₂ : formula L) = (u₁ =' u₂) ↔ t₁ = u₁ ∧ t₂ = u₂ :=
+⟨formula.equal.inj, by simp; exact congr_arg2 (=')⟩
 
 @[simp] lemma formula.imply.inj' (p₁ q₁ p₂ q₂ : formula L) : p₁ ⟶ p₂ = q₁ ⟶ q₂ ↔ p₁ = q₁ ∧ p₂ = q₂ :=
 ⟨formula.imply.inj, by simp; exact congr_arg2 (⟶)⟩
@@ -173,7 +173,7 @@ by simp[has_exists_quantifier.ex, formula.ex]
 @[simp] lemma formula.verum_ne_predicate {n} (r : L.pr n) (v : finitary (term L) n) :
   (⊤ : formula L) ≠ formula.app r v.
 
-@[simp] lemma formula.verum_ne_equal (t u : term L) : (⊤ : formula L) ≠ (t ≃ u).
+@[simp] lemma formula.verum_ne_equal (t u : term L) : (⊤ : formula L) ≠ (t =' u).
 
 @[simp] lemma formula.verum_ne_imply (p q : formula L) : ⊤ ≠ (p ⟶ q).
 
@@ -185,7 +185,7 @@ by simp[has_exists_quantifier.ex, formula.ex]
   formula.app r v ≠ ⊤.
 
 @[simp] lemma formula.predicate_ne_equal {n} (r : L.pr n) (v : finitary (term L) n) (t u : term L) :
-  formula.app r v ≠ (t ≃ u).
+  formula.app r v ≠ (t =' u).
 
 @[simp] lemma formula.predicate_ne_imply {n} (r : L.pr n) (v : finitary (term L) n) (p q : formula L) :
   formula.app r v ≠ p ⟶ q.
@@ -197,19 +197,19 @@ by simp[has_exists_quantifier.ex, formula.ex]
   formula.app r v ≠ ∀.p.
 
 @[simp] lemma formula.equal_ne_verum (t u : term L) :
-  (t ≃ u : formula L) ≠ ⊤.
+  (t =' u : formula L) ≠ ⊤.
 
 @[simp] lemma formula.equal_ne_predivate (t u : term L) {n} (r : L.pr n) (v : finitary (term L) n) :
-  (t ≃ u) ≠ formula.app r v.
+  (t =' u) ≠ formula.app r v.
 
 @[simp] lemma formula.equal_ne_imply (t u : term L) (p q : formula L) :
-  (t ≃ u) ≠ p ⟶ q.
+  (t =' u) ≠ p ⟶ q.
 
 @[simp] lemma formula.equal_ne_neg (t u : term L) (p : formula L) :
-  (t ≃ u) ≠ ∼p.
+  (t =' u) ≠ ∼p.
 
 @[simp] lemma formula.equal_ne_fal (t u : term L) (p : formula L) :
-  (t ≃ u : formula L) ≠ ∀.p.
+  (t =' u : formula L) ≠ ∀.p.
 
 @[simp] lemma formula.imply_ne_verum (p q : formula L) :
   p ⟶ q ≠ ⊤.
@@ -218,7 +218,7 @@ by simp[has_exists_quantifier.ex, formula.ex]
   p ⟶ q ≠ formula.app r v.
 
 @[simp] lemma formula.imply_ne_equal (p q : formula L) (t u : term L) :
-  p ⟶ q ≠ (t ≃ u).
+  p ⟶ q ≠ (t =' u).
 
 @[simp] lemma formula.imply_ne_neg (p q r : formula L) : p ⟶ q ≠ ∼r.
 
@@ -229,7 +229,7 @@ by simp[has_exists_quantifier.ex, formula.ex]
 @[simp] lemma formula.neg_ne_predicate (p : formula L) {n} (r : L.pr n) (v : finitary (term L) n) :
  ∼p ≠ formula.app r v.
 
-@[simp] lemma formula.neg_ne_equal (p : formula L) (t u : term L) : ∼p ≠ (t ≃ u).
+@[simp] lemma formula.neg_ne_equal (p : formula L) (t u : term L) : ∼p ≠ (t =' u).
 
 @[simp] lemma formula.neg_ne_imply (p q r : formula L) : ∼p ≠ (q ⟶ r).
 
@@ -242,7 +242,7 @@ by simp[has_exists_quantifier.ex, formula.ex]
   ∀.p ≠ formula.app r v.
 
 @[simp] lemma formula.fal_ne_equal (p : formula L) (t u : term L) :
-  (∀.p : formula L) ≠ (t ≃ u).
+  (∀.p : formula L) ≠ (t =' u).
 
 @[simp] lemma formula.fal_ne_imp (p q r : formula L) : (∀.p : formula L) ≠ (q ⟶ r).
 
@@ -670,7 +670,7 @@ lemma rewriting_sf_perm {s : ℕ → term L} (h : ∀ n, ∃ m, s m = #n) : ∀ 
 @[simp] def formula.arity : formula L → ℕ
 | ⊤                 := 0
 | (formula.app p v) := ⨆ᶠ i, (v i).arity
-| (t ≃ u)          := max t.arity u.arity
+| (t =' u)          := max t.arity u.arity
 | (p ⟶ q)           := max p.arity q.arity
 | (∼p)              := p.arity
 | (∀.p)             := p.arity - 1
@@ -738,7 +738,7 @@ by unfold has_elem.elem; simp
 @[simp] def rew : (ℕ → term L) → formula L → formula L
 | s ⊤         := ⊤
 | s (app p v) := app p (λ i, (v i).rew s)
-| s (t ≃ u)  := (t.rew s) ≃ (u.rew s)
+| s (t =' u)  := (t.rew s) =' (u.rew s)
 | s (p ⟶ q)  := p.rew s ⟶ q.rew s
 | s (∼p)      := ∼(p.rew s)
 | s (∀.p)   := ∀.(p.rew (s^1))
@@ -776,12 +776,12 @@ by { induction i with i IH generalizing s, { simp },
 @[simp] lemma rew_id (p : formula L) : p.rew ı = p :=
 by { induction p; try { simp[rew] }; try {simp*} }
 
-@[simp] lemma inf_conjunction_rew {n} (P : finitary (formula L) n) (s) :
-  (inf_conjunction n P).rew s = ⋀ i, (P i).rew s :=
+@[simp] lemma finitary.conjunction_rew {n} (P : finitary (formula L) n) (s) :
+  (finitary.conjunction n P).rew s = ⋀ i, (P i).rew s :=
 by { induction n with n IH; simp* }
 
-@[simp] lemma sup_disjunction_rew {n} (P : finitary (formula L) n) (s) :
-  (sup_disjunction n P).rew s = ⋁ i, (P i).rew s :=
+@[simp] lemma finitary.disjunction_rew {n} (P : finitary (formula L) n) (s) :
+  (finitary.disjunction n P).rew s = ⋁ i, (P i).rew s :=
 by { induction n with n IH; simp* }
 
 instance : has_pow (formula L) ℕ := ⟨λ p i, p.rew (λ x, #(x + i))⟩
@@ -812,14 +812,14 @@ by simp[pow_eq]; refl
 
 @[simp] lemma top_pow (i : ℕ) : (⊤ : formula L)^i = ⊤ := by refl
 @[simp] lemma bot_pow (i : ℕ) : (⊥ : formula L)^i = ⊥ := by refl
-@[simp] lemma eq_pow (t u : term L) (i : ℕ) : (t ≃ u : formula L)^i = (t^i ≃ u^i) := rfl
+@[simp] lemma eq_pow (t u : term L) (i : ℕ) : (t =' u : formula L)^i = (t^i =' u^i) := rfl
 @[simp] lemma imply_pow (p q : formula L) (i : ℕ) : (p ⟶ q)^i = p^i ⟶ q^i := rfl
 @[simp] lemma neg_pow (p : formula L) (i : ℕ) : (∼p)^i = ∼(p^i) := rfl
 @[simp] lemma and_pow (p q : formula L) (i : ℕ) : (p ⊓ q)^i = (p^i) ⊓ (q^i) := rfl
-@[simp] lemma inf_conjunction_pow {n} (P : finitary (formula L) n) (i : ℕ) : (inf_conjunction n P)^i = ⋀ j, (P j)^i :=
+@[simp] lemma finitary.conjunction_pow {n} (P : finitary (formula L) n) (i : ℕ) : (finitary.conjunction n P)^i = ⋀ j, (P j)^i :=
 by induction n with n IH; simp*
 @[simp] lemma or_pow (p q : formula L) (i : ℕ) : (p ⊔ q)^i = (p^i) ⊔ (q^i) := rfl
-@[simp] lemma sup_disjunction_pow {n} (P : finitary (formula L) n) (i : ℕ) : (sup_disjunction n P)^i = ⋁ j, (P j)^i :=
+@[simp] lemma finitary.disjunction_pow {n} (P : finitary (formula L) n) (i : ℕ) : (finitary.disjunction n P)^i = ⋁ j, (P j)^i :=
 by induction n with n IH; simp*
 
 lemma fal_pow (p : formula L) (i : ℕ) : (∀.p)^i = ∀.p.rew (#0 ⌢ λ x, #(x + i + 1)) :=
@@ -840,7 +840,7 @@ lemma nested_rew : ∀ (p : formula L) (s₀ s₁),
   (p.rew s₀).rew s₁ = p.rew (λ x, (s₀ x).rew s₁)
 | ⊤         _ _ := by simp
 | (❴p❵ v) _ _ := by simp[rew]
-| (t ≃ u)  _ _ := by simp[rew]
+| (t =' u)  _ _ := by simp[rew]
 | (p ⟶ q)   _ _ := by simp[rew, nested_rew p, nested_rew q]
 | (∼p)      _ _ := by simp[rew]; refine nested_rew p _ _
 | (∀.p)     _ _ := by { simp[rew, nested_rew p], congr,
@@ -851,7 +851,7 @@ lemma rew_rew : ∀ (p : formula L) {s₀ s₁ : ℕ → term L},
 | ⊤         _ _ _ := by simp
 | (❴p❵ v) _ _ h := by simp[rew, arity] at h ⊢; refine funext
     (λ i, term.rew_rew (v i) (λ m eqn, h _ $ lt_of_lt_of_le eqn (le_fintype_sup _ i)))
-| (t ≃ u)  _ _ h := by simp[rew, arity] at h ⊢;
+| (t =' u)  _ _ h := by simp[rew, arity] at h ⊢;
     { refine ⟨term.rew_rew _ (λ _ e, h _ (or.inl e)), term.rew_rew _ (λ _ e, h _ (or.inr e))⟩ }
 | (p ⟶ q)   _ _ h := by simp[rew, arity] at h ⊢;
     refine ⟨rew_rew _ (λ _ e, h _ (or.inl e)), rew_rew _ (λ _ e, h _ (or.inr e))⟩
@@ -892,9 +892,9 @@ lemma total_rew_inv :
 | _ _ ⊤              := ⟨⊤, by simp⟩
 | s h (@app _ n p v) := by rcases classical.skolem.mp (λ i : fin n, @term.total_rew_inv _ s h (v i : term L)) with ⟨w, w_p⟩;
     refine ⟨❴p❵ w, by simp[w_p]⟩
-| s h (t ≃ u)       := 
+| s h (t =' u)       := 
     by rcases term.total_rew_inv s h t with ⟨w₁, e_w₁⟩;
-       rcases term.total_rew_inv s h u with ⟨w₂, e_w₂⟩; refine ⟨w₁ ≃ w₂, by simp[e_w₁, e_w₂]⟩
+       rcases term.total_rew_inv s h u with ⟨w₂, e_w₂⟩; refine ⟨w₁ =' w₂, by simp[e_w₁, e_w₂]⟩
 | s h (p ⟶ q)        := 
     by rcases total_rew_inv s h p with ⟨p', e_p'⟩;
        rcases total_rew_inv s h q with ⟨q', e_q'⟩; refine ⟨p' ⟶ q', by simp*⟩
@@ -912,18 +912,18 @@ lemma total_rew_inv :
       have : term.rew_var s (v₁ i) = term.rew_var s (v₂ i), from congr_fun h i,
       exact (term.rew_var_inj_of_inj I).mp this },
     { rintros rfl, simp } }
-| (formula.app p v)   (t ≃ u)            s I := by simp[rew_var]
+| (formula.app p v)   (t =' u)            s I := by simp[rew_var]
 | (formula.app r v)   (p ⟶ q)             s I := by simp[rew_var]
 | (formula.app r v)   (∼p)                s I := by simp[rew_var]
 | (formula.app r v)   (∀.p)               s I := by simp[rew_var, fal_pow]
-| (t ≃ u)            p                   s I := by cases p; simp[rew_var, fal_pow, I]
+| (t =' u)            p                   s I := by cases p; simp[rew_var, fal_pow, I]
 | (p ⟶ q)             r                   s I :=
     by cases r; simp[rew_var, fal_pow, @rew_var_inj_of_inj p _ s I, @rew_var_inj_of_inj q _ s I]
 | (∼p)                q                   s I :=
     by cases q; simp[rew_var, fal_pow, @rew_var_inj_of_inj p _ s I]
 | (∀.p)               ⊤                   s I := by simp[rew_var]
 | (∀.p)               (formula.app r v)   s I := by simp[rew_var]
-| (∀.p)               (t ≃ u)            s I := by simp[rew_var]
+| (∀.p)               (t =' u)            s I := by simp[rew_var]
 | (∀.p)               (q ⟶ r)             s I := by simp[rew_var]
 | (∀.p)               (∼q)                s I := by simp[rew_var]
 | (∀.p)               (∀.q)               s I := by {simp[rew_var, fal_pow], 
@@ -941,7 +941,7 @@ lemma total_rew_inv :
 @[simp] def is_open : Theory L
 | ⊤          := true
 | (❴p❵ v)  := true
-| (t ≃ u)   := true
+| (t =' u)   := true
 | (p ⟶ q)    := p.is_open ∧ q.is_open
 | (∼p)       := p.is_open
 | (∀.p)      := false
@@ -957,7 +957,7 @@ lemma total_rew_inv :
 @[simp] def is_open_rew : ∀ {p : formula L} {s}, (p.rew s).is_open ↔ p.is_open
 | ⊤        s := by simp
 | (❴p❵ v)  s := by simp
-| (t ≃ u) s := by simp
+| (t =' u) s := by simp
 | (p ⟶ q) s  := by simp[@is_open_rew p s, @is_open_rew q s]
 | (∼p)     s := by simp[@is_open_rew p s]
 | (∀.p)  s   := by simp
@@ -977,7 +977,7 @@ lemma nfal_is_sentence (p : formula L) : is_sentence (nfal p p.arity) :=
 by simp[is_sentence]
 
 @[simp] lemma conjunction_arity {n} {v : finitary (formula L) n} :
-  (inf_conjunction n v).arity = ⨆ᶠ i, (v i).arity :=
+  (finitary.conjunction n v).arity = ⨆ᶠ i, (v i).arity :=
 by { induction n with n IH; simp*,
   refine le_antisymm _ _; simp,
   { split,
@@ -994,7 +994,7 @@ by { induction n with n IH; simp*,
       { refl }, { refine le_trans _ le, refine le_fintype_sup' ⟨i, lt⟩ (by refl) } } } }
 
 @[simp] lemma disjunction_arity {n} {v : finitary (formula L) n} :
-  (sup_disjunction n v).arity = ⨆ᶠ i, (v i).arity :=
+  (finitary.disjunction n v).arity = ⨆ᶠ i, (v i).arity :=
 by { induction n with n IH; simp*,
   refine le_antisymm _ _; simp,
   { split,
@@ -1087,7 +1087,7 @@ end
 @[simp] def fn_symbols : formula L → set (Σ n, L.fn n)
 | ⊤         := ∅
 | (app r v) := ⋃ i, (v i).symbols
-| (t ≃ u)  := t.symbols ∪ u.symbols
+| (t =' u)  := t.symbols ∪ u.symbols
 | (p ⟶ q)   := fn_symbols p ∪ q.fn_symbols
 | (∼p)      := p.fn_symbols
 | (∀.p)     := p.fn_symbols
@@ -1101,7 +1101,7 @@ by simp[fn_symbols']
 @[simp] def pr_symbols : formula L → set (Σ n, L.pr n)
 | ⊤         := ∅
 | (app r v) := {⟨_, r⟩}
-| (t ≃ u)  := ∅
+| (t =' u)  := ∅
 | (p ⟶ q)   := p.pr_symbols ∪ q.pr_symbols
 | (∼p)      := p.pr_symbols
 | (∀.p)     := p.pr_symbols
@@ -1115,7 +1115,7 @@ by simp[pr_symbols']
 lemma fn_symbols_finite : ∀ p : formula L, p.fn_symbols.finite
 | ⊤         := by simp
 | (app r v) := set.finite_Union (λ i, (v i).symbols_finite)
-| (t ≃ u)  := set.finite.union t.symbols_finite u.symbols_finite
+| (t =' u)  := set.finite.union t.symbols_finite u.symbols_finite
 | (p ⟶ q)   := set.finite.union p.fn_symbols_finite q.fn_symbols_finite
 | (∼p)      := p.fn_symbols_finite
 | (∀.p)     := p.fn_symbols_finite
@@ -1127,7 +1127,7 @@ by { have : p.fn_symbols' n = (λ f : L.fn n, (⟨n, f⟩ : Σ n, L.fn n))⁻¹'
 lemma pr_symbols_finite : ∀ p : formula L, p.pr_symbols.finite
 | ⊤         := by simp
 | (app r v) := by simp
-| (t ≃ u)  := by simp
+| (t =' u)  := by simp
 | (p ⟶ q)   := set.finite.union p.pr_symbols_finite q.pr_symbols_finite
 | (∼p)      := p.pr_symbols_finite
 | (∀.p)     := p.pr_symbols_finite
@@ -1145,7 +1145,7 @@ inductive subformula : formula L → formula L → Prop
 @[simp] def complexity : formula L → ℕ
 | ⊤         := 0
 | (app r v) := 0
-| (t ≃ u)  := 0
+| (t =' u)  := 0
 | (∼p)      := p.complexity + 1
 | (p ⟶ q)  := max p.complexity q.complexity + 1
 | (∀.p)     := p.complexity + 1
@@ -1153,19 +1153,17 @@ inductive subformula : formula L → formula L → Prop
 instance : wf_lt (formula L) :=
 { prelt := subformula,
   wt := complexity,
-  mono' := λ a b h, by { induction h; try { simp },
-  case implyl : p q { exact nat.lt_succ_iff.mpr (le_max_left p.complexity q.complexity) },
-  case implyr : p q { exact nat.lt_succ_iff.mpr (le_max_right p.complexity q.complexity) } } }
+  mono' := λ a b h, by induction h; simp }
 
 @[simp] lemma lt_app {p : formula L} {n} {r : L.pr n} {v} : ¬p < app r v :=
 by { simp [wf_lt.lt_iff], intros p h, rcases h }
 
 @[simp] lemma le_app {p : formula L} {n} {r : L.pr n} {v} : p ≤ app r v ↔ p = app r v := by simp[le_iff_lt_or_eq]
 
-@[simp] lemma lt_equal {p : formula L} {t u : term L} : ¬p < (t ≃ u) :=
+@[simp] lemma lt_equal {p : formula L} {t u : term L} : ¬p < (t =' u) :=
 by { simp [wf_lt.lt_iff], intros p h, rcases h }
 
-@[simp] lemma le_equal {p : formula L} {t u : term L} : p ≤ (t ≃ u) ↔ p = (t ≃ u) := by simp[le_iff_lt_or_eq]
+@[simp] lemma le_equal {p : formula L} {t u : term L} : p ≤ (t =' u) ↔ p = (t =' u) := by simp[le_iff_lt_or_eq]
 
 @[simp] lemma lt_verum {p : formula L} : ¬p < ⊤ :=
 by { simp [wf_lt.lt_iff], intros p h, rcases h }
@@ -1236,16 +1234,16 @@ by { induction h; try { simp },
 
 inductive subterm : term L → formula L → Prop
 | app    : ∀ {n} (r : L.pr n) (v : finitary (term L) n) (i), subterm (v i) (app r v)
-| equall : ∀ {t u : term L}, subterm t (t ≃ u)
-| equalr : ∀ {t u : term L}, subterm u (t ≃ u)
+| equall : ∀ {t u : term L}, subterm t (t =' u)
+| equalr : ∀ {t u : term L}, subterm u (t =' u)
 
 instance : has_mem (term L) (formula L) := ⟨λ t p, ∃ (t' ≥ t) (p' ≤ p), subterm t' p'⟩
 
 lemma mem_def {t : term L} {p : formula L} : t ∈ p ↔ ∃ (t' ≥ t) (p' ≤ p), subterm t' p' := by refl
 
-@[simp] lemma mem_equall (t u : term L) : t ∈ (t ≃ u : formula L) := ⟨t, by simp, t ≃ u, by simp, subterm.equall⟩ 
+@[simp] lemma mem_equall (t u : term L) : t ∈ (t =' u : formula L) := ⟨t, by simp, t =' u, by simp, subterm.equall⟩ 
 
-@[simp] lemma mem_equalr (t u : term L) : u ∈ (t ≃ u : formula L) := ⟨u, by simp, t ≃ u, by simp, subterm.equalr⟩ 
+@[simp] lemma mem_equalr (t u : term L) : u ∈ (t =' u : formula L) := ⟨u, by simp, t =' u, by simp, subterm.equalr⟩ 
 
 lemma mem_of_formula_le_mem {t : term L} {p q : formula L} : t ∈ p → p ≤ q → t ∈ q :=
 by { rintros ⟨t', ht', p', hp', sb⟩ le, refine ⟨t', ht', p', (le_trans hp' le), sb⟩ }
@@ -1261,13 +1259,13 @@ by { rintros ⟨t', ht', p', hp', sb⟩ le, refine ⟨t', le_trans le ht', p', h
  by { rintros ⟨i, le⟩, refine mem_of_term_le_mem ⟨v i, by simp, app r v, by simp, subterm.app r v i⟩ le }⟩
 
 @[simp] lemma mem_equal {s t u : term L} :
-  s ∈ (t ≃ u : formula L) ↔ s ≤ t ∨ s ≤ u :=
+  s ∈ (t =' u : formula L) ↔ s ≤ t ∨ s ≤ u :=
 ⟨by { rintros ⟨t', ht', p', hp', sb⟩,
-      have hp' : p' = (t ≃ u) ∨ p' < (t ≃ u), exact eq_or_lt_of_le hp', simp at hp',
+      have hp' : p' = (t =' u) ∨ p' < (t =' u), exact eq_or_lt_of_le hp', simp at hp',
       rcases hp' with rfl, cases sb, { exact or.inl ht' }, { exact or.inr ht' } },
  by { rintros (le | le),
-      { refine mem_of_term_le_mem ⟨t, by simp, t ≃ u, by simp, subterm.equall⟩ le },
-      { refine mem_of_term_le_mem ⟨u, by simp, t ≃ u, by simp, subterm.equalr⟩ le } }⟩
+      { refine mem_of_term_le_mem ⟨t, by simp, t =' u, by simp, subterm.equall⟩ le },
+      { refine mem_of_term_le_mem ⟨u, by simp, t =' u, by simp, subterm.equalr⟩ le } }⟩
 
 @[simp] lemma mem_verum {t : term L} :
   ¬t ∈ (⊤ : formula L) :=
@@ -1353,7 +1351,7 @@ begin
   induction p,
   case verum { have : {q : formula L | q.subformula ⊤} = ∅, { ext q, simp, intros h, rcases h }, simp[this] },
   case app : n r v { have : {q : formula L | q.subformula (app r v)} = ∅, { ext q, simp, intros h, rcases h }, simp[this] },
-  case equal : t u { have : {q : formula L | q.subformula (t ≃ u)} = ∅, { ext q, simp, intros h, rcases h }, simp[this] },
+  case equal : t u { have : {q : formula L | q.subformula (t =' u)} = ∅, { ext q, simp, intros h, rcases h }, simp[this] },
   case imply : p q { have : {r : formula L | r.subformula (p ⟶ q)} = {p, q},
     { ext r, simp, split, { rintros h, rcases h; simp }, { rintros (rfl | rfl), exact subformula.implyl, exact subformula.implyr } },
     simp[this] },
@@ -1380,7 +1378,7 @@ begin
       { intros h, rcases h, simp }, { rintros ⟨i, rfl⟩, exact subterm.app r v i } },
     simp[this, set.finite_range] },
   case equal : t u
-  { have : {s : term L | subterm s (t ≃ u)} = {t, u},
+  { have : {s : term L | subterm s (t =' u)} = {t, u},
     { ext s, simp, split,
       { intros h, rcases h; simp }, { rintros (rfl | rfl), exact subterm.equall, exact subterm.equalr } },
     simp[this] },
